refactor

src/drf/DRF_PF3.v
@@ -35,1934 +35,638 @@ Require Import ReorderPromises2.
 
 Require Import DRF_PF0.
 Require Import DRF_PF1.
-Require Import DRF_PF4.
-Require Import Mapping.
 
 Require Import PFConsistent.
 
 Set Implicit Arguments.
 
-Definition collapsing_latest_reserves (L: Loc.t -> Prop)
-           (mem: Memory.t) (loc: Loc.t) (to: Time.t) (from: Time.t) :=
-  (<<LATEST: to = Memory.max_ts loc mem>>) /\
-  (<<RESERVE: Memory.get loc to mem = Some (from, Message.reserve)>>) /\
-  (<<OTHER: L loc>>)
-.
 
-Definition collapsing_latest_reserves_times (L: Loc.t -> Prop)
-           (mem: Memory.t) (loc: Loc.t) (to: Time.t): Prop :=
-  exists from,
-    (<<RESERVE: collapsing_latest_reserves L mem loc to from>>).
+Section CANCEL.
 
-Definition collapsing_caps (L: Loc.t -> Prop)
-           (mem0 mem1: Memory.t) (loc: Loc.t) (to: Time.t) (from: Time.t) :=
-  (<<LATEST: exists val released,
-      (<<CAP: caps mem0 mem1 loc to from (Message.full val released)>>)>>) /\
-  (<<OTHER: L loc>>)
-.
+  Inductive only_reserves (proms: Memory.t): Prop :=
+  | only_reserves_intro
+      (RESERVES: forall loc to from msg (GET: Memory.get loc to proms = Some (from, msg)),
+          msg = Message.reserve)
+      (FINITE: Memory.finite proms)
+  .
 
-Definition collapsing_caps_times (L: Loc.t -> Prop)
-           (mem0 mem1: Memory.t) (loc: Loc.t) (to: Time.t) :=
-  exists from,
-    (<<CAP: collapsing_caps L mem0 mem1 loc to from>>).
-
-Inductive caps_collapsing (L: Loc.t -> Prop)
-          (mem: Memory.t): Loc.t -> Time.t -> Time.t -> Prop :=
-| caps_collapsing_not_in
-    loc t
-    (NSAT: ~ L loc)
-  :
-    caps_collapsing L mem loc t t
-| caps_collapsing_in_memory
-    loc t max
-    (SAT: L loc)
-    (FULL: Memory.max_full_ts mem loc max)
-    (TLE: Time.le t max)
-  :
-    caps_collapsing L mem loc t t
-| caps_collapsing_cap
-    loc t max
-    (SAT: L loc)
-    (FULL: Memory.max_full_ts mem loc max)
-    (TS0: Time.lt max t)
-    (TS1: Time.le t (Time.incr (Memory.max_ts loc mem)))
-  :
-    caps_collapsing L mem loc t max
-| caps_collapsing_outer_memory
-    loc t
-    (SAT: L loc)
-    (TLE: Time.lt (Time.incr (Memory.max_ts loc mem)) t)
-  :
-    caps_collapsing L mem loc t t
-.
-
-Lemma caps_get_reserve mem0 prom mem1 loc to from
-      (RESERVE: Memory.reserve_wf prom mem0)
-      (CLOSED: Memory.closed mem0)
-      (CAP: Memory.cap prom mem0 mem1)
-      (CAPS: caps mem0 mem1 loc to from Message.reserve)
-  :
-    exists from0 to1 msg0 msg1,
-      (<<GET0: Memory.get loc from mem0 = Some (from0, msg0)>>) /\
-      (<<GET1: Memory.get loc to1 mem0 = Some (to, msg1)>>) /\
-      (<<SPACE: forall t (ITV: Interval.mem (from, to) t), ~ covered loc t mem0>>)
-.
-Proof.
-  unfold caps in CAPS. des. inv CAP.
-  exploit COMPLETE; eauto. i. des.
-  set (@cell_elements_least
-         (mem0 loc)
-         (fun t => Time.lt from t)). des.
-  - hexploit (MIDDLE loc f from from0 to0).
-    { econs; eauto. i.
-      destruct (Memory.get loc ts mem0) eqn:GET2; auto. destruct p.
-      exfalso. exploit LEAST.
-      - eapply GET2.
-      - eauto.
-      - i. exploit Memory.get_ts; try apply GET.
-        i. des; clarify.
-        + eapply Time.lt_strorder. eapply TimeFacts.lt_le_lt.
-          * eapply SAT.
-          * eapply Time.bot_spec.
-        + eapply Time.lt_strorder. eapply TimeFacts.le_lt_lt.
-          * etrans.
-            { eapply x1. }
-            { eapply TS2. }
-          * eauto. }
-    { exploit memory_get_from_mon.
-      - eapply x.
-      - eapply GET.
-      - eauto.
-      - i. destruct x2; auto. destruct H. exfalso.
-        exploit memory_get_from_inj.
-        { eapply SOUND. eapply GET. }
-        { eapply GET1. }
-        i. des; clarify.
-        + setoid_rewrite GET0 in GET. clarify.
-        + eapply Time.lt_strorder; eauto. }
-    i. exploit memory_get_from_inj.
-    { eapply H. }
-    { eapply GET1. }
-    i. des; clarify.
-    + esplits; eauto. ii. inv H0.
-      exploit Memory.get_disjoint.
-      * eapply SOUND. eapply GET2.
-      * eapply H.
-      * i. des; clarify. eapply x2; eauto.
-    + inv CLOSED. specialize (INHABITED loc).
-      eapply SOUND in INHABITED. clarify.
-  - exploit Memory.max_ts_spec.
-    { eapply x. }
-    i. des. destruct MAX.
-    + exfalso. eapply EMPTY; eauto.
-    + unfold Time.eq in *. subst. exploit x0; auto. intros LATEST.
-      exploit Memory.latest_val_exists; eauto.
-      { inv CLOSED. eauto. }
-      i. des.
-      exploit Memory.max_full_view_exists; eauto.
-      { inv CLOSED. eauto. } i. des.
-      exploit BACK; eauto. i.
-      exploit memory_get_from_inj.
-      * eapply x1.
-      * eapply GET1.
-      * i. des; clarify.
-        { exfalso. eapply Time.lt_strorder. eapply TimeFacts.lt_le_lt.
-          - eapply Time.incr_spec.
-          - rewrite BOT0. eapply Time.bot_spec. }
-        { inv CLOSED. erewrite INHABITED in GET0. clarify. }
-Qed.
-
-Lemma max_full_ts_not_collapsed L prom mem0 mem1 loc max
-      (INHABITED: Memory.inhabited mem0)
-      (CAP: Memory.cap prom mem0 mem1)
-      (MAX: Memory.max_full_ts mem0 loc max)
-  :
-    ~ (collapsing_latest_reserves_times L mem0 \2/ collapsing_caps_times L mem0 mem1) loc max.
-Proof.
-  ii. des.
-  - inv H. inv H0. des. clarify.
-    exploit Memory.max_full_ts_spec; eauto. i. des. clarify.
-  - inv H. inv H0. des. inv CAP0.
-    exploit Memory.max_full_ts_spec; eauto. i. des. clarify.
-Qed.
-
-Definition memory_concrete_le (lhs rhs: Memory.t): Prop :=
-  forall loc to from val released
-         (GET: Memory.get loc to lhs = Some (from, Message.full val released)),
-    Memory.get loc to rhs = Some (from, Message.full val released).
-Global Program Instance le_PreOrder: PreOrder memory_concrete_le.
-Next Obligation. ii. ss. Qed.
-Next Obligation. ii. eauto. Qed.
-
-Lemma memory_concrete_le_le
-  :
-    Memory.le <2= memory_concrete_le.
-Proof.
-  ii. eauto.
-Qed.
-Hint Resolve memory_concrete_le_le.
-
-Lemma memory_concrete_le_closed_timemap tm mem0 mem1
-      (MLE: memory_concrete_le mem0 mem1)
-      (TM: Memory.closed_timemap tm mem0)
-  :
-    Memory.closed_timemap tm mem1.
-Proof.
-  ii. hexploit (TM loc). i. des.
-  esplits; eauto.
-Qed.
-
-Lemma memory_concrete_le_closed_view vw mem0 mem1
-      (MLE: memory_concrete_le mem0 mem1)
-      (VW: Memory.closed_view vw mem0)
-  :
-    Memory.closed_view vw mem1.
-Proof.
-  inv VW. econs.
-  - eapply memory_concrete_le_closed_timemap; eauto.
-  - eapply memory_concrete_le_closed_timemap; eauto.
-Qed.
-
-Lemma memory_concrete_le_closed_opt_view vw mem0 mem1
-      (MLE: memory_concrete_le mem0 mem1)
-      (VW: Memory.closed_opt_view vw mem0)
-  :
-    Memory.closed_opt_view vw mem1.
-Proof.
-  inv VW; econs.
-  eapply memory_concrete_le_closed_view; eauto.
-Qed.
-
-Lemma memory_concrete_le_closed_msg msg mem0 mem1
-      (MLE: memory_concrete_le mem0 mem1)
-      (MSG: Memory.closed_message msg mem0)
-  :
-    Memory.closed_message msg mem1.
-Proof.
-  inv MSG; econs.
-  eapply memory_concrete_le_closed_opt_view; eauto.
-Qed.
-
-Lemma memory_concrete_le_closed_tview vw mem0 mem1
-      (MLE: memory_concrete_le mem0 mem1)
-      (VW: TView.closed vw mem0)
-  :
-    TView.closed vw mem1.
-Proof.
-  inv VW. econs.
-  - i. eapply memory_concrete_le_closed_view; eauto.
-  - eapply memory_concrete_le_closed_view; eauto.
-  - eapply memory_concrete_le_closed_view; eauto.
-Qed.
-
-Lemma memory_concrete_le_reserve_wf prom mem0 mem1
-      (MLE: memory_concrete_le mem0 mem1)
-      (RESERVE: Memory.reserve_wf prom mem0)
-  :
-    Memory.reserve_wf prom mem1.
-Proof.
-  ii. eapply RESERVE in GET. des.
-  esplits; eauto.
-Qed.
-
-Lemma memory_concrete_le_local_wf lc mem0 mem1
-      (MLE: memory_concrete_le mem0 mem1)
-      (PROM: Memory.le (Local.promises lc) mem1)
-      (LOCAL: Local.wf lc mem0)
-  :
-    Local.wf lc mem1.
-Proof.
-  inv LOCAL. econs; eauto.
-  - eapply memory_concrete_le_closed_tview; eauto.
-  - eapply memory_concrete_le_reserve_wf; eauto.
-Qed.
-
-Lemma partial_cap_closed prom mem0 mem1 mem2
-      (MLE: Memory.le prom mem0)
-      (CLOSED: Memory.closed mem0)
-      (RESERVEWF: Memory.reserve_wf prom mem0)
-      (CAP: Memory.cap prom mem0 mem2)
-      (MLE0: Memory.le mem0 mem1)
-      (MLE1: Memory.le mem1 mem2)
-  :
-    Memory.closed mem1.
-Proof.
-  exploit Memory.max_full_timemap_exists; eauto.
-  { inv CLOSED. auto. }
-  intros [tm MAX].
-  inv CLOSED. econs; eauto.
-  i. destruct (Memory.get loc to mem0) as [[from0 msg0]|] eqn:GET.
-  - dup GET. eapply MLE0 in GET. clarify.
-    eapply CLOSED0 in GET0. des. esplits; eauto.
-    eapply memory_concrete_le_closed_msg; eauto.
-  - destruct msg.
-    + eapply MLE1 in MSG.
-      exploit caps_max_view; eauto.
-      * econs; eauto.
-      * i. des; clarify. esplits; eauto.
-        { econs; eauto. econs; eauto. econs. refl. }
-        { econs; eauto. ss. transitivity (Memory.max_ts loc mem0).
-          - specialize (MAX loc). inv MAX. des.
-            eapply Memory.max_ts_spec in GET0. des. eauto.
-          - left. eapply Time.incr_spec. }
-        { eapply memory_concrete_le_closed_msg; eauto.
-          econs. econs. econs.
-          - eapply Memory.max_full_timemap_closed; eauto.
-          - eapply Memory.max_full_timemap_closed; eauto. }
-    + esplits; eauto. econs.
-Qed.
-
-Lemma collapsing_caps_forget_le
-      mem0 mem1 mem2 prom (L: Loc.t -> Prop)
-      (CAP: Memory.cap prom mem0 mem2)
-      (FORGET: forget_memory (collapsing_latest_reserves_times L mem0 \2/ collapsing_caps_times L mem0 mem2) mem1 mem2)
-  :
-    memory_concrete_le mem0 mem1.
-Proof.
-  inv FORGET. ii.
-  erewrite COMPLETE.
-  - eapply Memory.cap_le in CAP; eauto. refl.
-  - ii. des.
-    + unfold collapsing_latest_reserves_times in *. des.
-      inv RESERVE. des. clarify.
-    + unfold collapsing_caps_times in *. des.
-      inv CAP0. des. unfold caps in CAP0. des. clarify.
-Qed.
-
-Definition collapsable_cap (L: Loc.t -> Prop) (prom mem: Memory.t): Prop :=
-  forall
-    loc (SAT: L loc)
-    from msg
-    (GET: Memory.get loc (Memory.max_ts loc mem) prom = Some (from, msg)),
-    msg <> Message.reserve.
-
-Lemma collapsing_caps_forget_prom_le
-      mem0 mem1 mem2 prom (L: Loc.t -> Prop)
-      (COLLAPSABLE: collapsable_cap L prom mem0)
-      (MLE: Memory.le prom mem0)
-      (CLOSED: Memory.closed mem0)
-      (RESERVEWF: Memory.reserve_wf prom mem0)
-      (CAP: Memory.cap prom mem0 mem2)
-      (FORGET: forget_memory (collapsing_latest_reserves_times L mem0 \2/ collapsing_caps_times L mem0 mem2) mem1 mem2)
-  :
-    Memory.le prom mem1.
-Proof.
-  inv FORGET. ii.
-  erewrite COMPLETE.
-  - eapply Memory.cap_le in CAP; eauto.
-  - ii. des.
-    + unfold collapsing_latest_reserves_times in *. des.
-      inv RESERVE. des. clarify.
-      dup LHS. eapply MLE in LHS0. clarify.
-      eapply COLLAPSABLE in OTHER. eapply OTHER in LHS. clarify.
-    + unfold collapsing_caps_times in *. des.
-      inv CAP0. des. unfold caps in CAP0. des.
-      eapply MLE in LHS; eauto. clarify.
-Qed.
-
-Lemma identity_mapped_view tm maxmap (f: Loc.t -> Time.t -> Time.t -> Prop)
-      (TM: TimeMap.le tm maxmap)
-      (IDENT: forall loc ts (TS: Time.le ts (maxmap loc)), f loc ts ts)
-  :
-    timemap_map f tm tm.
-Proof.
-  ii. eapply IDENT; eauto.
-Qed.
-
-Lemma caps_collapsing_ident L mem loc maxts ts
-      (MAX: Memory.max_full_ts mem loc maxts)
-      (TS: Time.le ts maxts)
-  :
-    (caps_collapsing L mem) loc ts ts.
-Proof.
-  i. destruct (classic (L loc)).
-  - econs 2; eauto.
-  - econs 1; eauto.
-Qed.
-
-Lemma not_latest_reserve_le_max_full_ts loc mem ts to from msg
-      (RESERVEWF : memory_reserve_wf mem)
-      (INHABITED : Memory.inhabited mem)
-      (MAX : Memory.max_full_ts mem loc ts)
-      (GET: Memory.get loc to mem = Some (from, msg))
-  :
-    (<<TLE: Time.le to ts>>) \/
-    ((<<TO: to = Memory.max_ts loc mem>>) /\
-     (<<FROM: from = ts>>) /\
-     (<<MSG: msg = Message.reserve>>)).
-Proof.
-  inv MAX. des.
-  destruct msg.
-  - left. eapply MAX0; eauto.
-  - exploit RESERVEWF; eauto. i. des.
-    destruct (TimeFacts.le_lt_dec to ts); auto.
-    dup x. eapply MAX0 in x; eauto. destruct x.
-    + exfalso. exploit memory_get_from_mon.
-      { eapply GET0. }
-      { eapply GET. }
-      { auto. }
-      i. eapply Time.lt_strorder. eapply TimeFacts.le_lt_lt.
-      * eapply x1.
-      * eapply H.
-    + unfold Time.eq in *. subst. right. esplits; eauto.
-      setoid_rewrite GET0 in x0. clarify.
-      dup GET. eapply Memory.max_ts_spec in GET1. des.
-      destruct MAX; auto. exfalso.
-      destruct msg.
-      * eapply MAX0 in GET2. eapply Time.lt_strorder.
-        eapply TimeFacts.lt_le_lt.
-        { etrans.
-          - eapply l.
-          - eapply H. }
+  Lemma reserves_cancelable lang st vw proms0 sc mem0
+        (FINITE: Memory.finite proms0)
+        (MLE: Memory.le proms0 mem0)
+    :
+      exists proms1 mem1,
+        (<<STEPS: rtc (tau (@pred_step is_cancel lang))
+                      (Thread.mk lang st (Local.mk vw proms0) sc mem0)
+                      (Thread.mk lang st (Local.mk vw proms1) sc mem1)>>) /\
+        (<<NORESERVES: no_reserves proms1>>).
+  Proof.
+    assert (exists dom,
+               (<<COMPLETE: forall loc to,
+                   (exists from, (<<GET: Memory.get loc to proms0 = Some (from, Message.reserve)>>))
+                   <-> (<<IN: List.In (loc, to) dom>>)>>)).
+    { unfold Memory.finite in *. des.
+      generalize (list_filter_exists (fun locto =>
+                                        match locto with
+                                        | (loc, to) =>
+                                          exists from, Memory.get loc to proms0 = Some (from, Message.reserve)
+                                        end) dom).
+      i. des. exists l'. split; i.
+      - eapply COMPLETE. des. esplits; eauto.
+      - eapply COMPLETE in H. des. esplits; eauto. }
+    des. ginduction dom; ss; i.
+    - exists proms0, mem0. esplits; eauto.
+      ii. clarify. eapply COMPLETE. eauto.
+    - destruct a as [loc to].
+      exploit (proj2 (COMPLETE loc to)); eauto. i. des.
+      destruct (classic (List.In (loc, to) dom)).
+      { exploit IHdom; eauto. i. split; i.
+        - des. exploit (proj1 (COMPLETE loc0 to0)); eauto.
+          i. des; clarify.
+        - exploit (proj2 (COMPLETE loc0 to0)); eauto. }
+      exploit Memory.remove_exists; eauto.
+      intros [prom1 REMOVE0].
+      exploit Memory.remove_exists.
+      { eapply MLE. eapply GET. }
+      intros [mem1 REMOVE1]. hexploit IHdom.
+      * instantiate (1:=prom1).
+        eapply Memory.remove_finite; eauto.
+      * instantiate (1:=mem1).
+        ii. erewrite Memory.remove_o in LHS; eauto. des_ifs.
+        eapply MLE in LHS. erewrite Memory.remove_o; eauto. des_ifs.
+        ss. des; clarify.
+      * i. split; i.
+        { des. erewrite Memory.remove_o in GET0; eauto. des_ifs.
+          exploit (proj1 (COMPLETE loc0 to0)); eauto. i. des; clarify. }
+        { exploit (proj2 (COMPLETE loc0 to0)); eauto. i. des; clarify.
+          exists from0. erewrite Memory.remove_o; eauto. des_ifs.
+          ss. des; clarify. }
+      * i. des. exists proms1, mem2. split; eauto.
+        econs 2.
+        { econs.
+          - instantiate (2:=ThreadEvent.promise loc from to Message.reserve Memory.op_kind_cancel).
+            econs; ss. econs. econs 1. econs; ss.
+            econs; ss. econs; eauto.
+          - eauto. }
         { eauto. }
-      * dup GET2. eapply RESERVEWF in GET2. des.
-        eapply MAX0 in GET2.
-        exploit memory_get_from_mon.
-        { eapply GET. }
-        { eapply GET1. }
-        { eapply H. }
-        i. eapply Time.lt_strorder.
-        eapply TimeFacts.lt_le_lt.
-        { eapply l. }
-        { etrans.
-          - eapply x0.
-          - eapply Memory.get_ts in GET1. des; clarify. }
-Qed.
+  Qed.
 
-Lemma caps_collapsing_ident2 L mem maxts loc ts fts
-      (MAX: Memory.max_full_ts mem loc maxts)
-      (TS: Time.le ts maxts)
-      (MAP: (caps_collapsing L mem) loc ts fts)
-  :
-    ts = fts.
-Proof.
-  inv MAP; eauto.
-  exploit Memory.max_full_ts_inj.
-  { eapply FULL. }
-  { eapply MAX. } i. clarify.
-  exfalso. eapply Time.lt_strorder. eapply TimeFacts.lt_le_lt.
-  { eapply TS0. }
-  { eapply TS. }
-Qed.
+  Lemma promise_not_cacncel_reserves_same prom0 mem0 loc from to msg prom1 mem1 kind
+        (PROM: Memory.promise prom0 mem0 loc from to msg prom1 mem1 kind)
+        (NOTCANCEL: kind <> Memory.op_kind_cancel)
+        loc0 to0 from0
+        (GET: Memory.get loc0 to0 prom0 = Some (from0, Message.reserve))
+    :
+      exists from1,
+        Memory.get loc0 to0 prom1 = Some (from1, Message.reserve).
+  Proof.
+    inv PROM.
+    - eapply Memory.add_get1 in GET; eauto.
+    - des. clarify. erewrite Memory.split_o; eauto.
+      dup PROMISES. eapply Memory.split_get0 in PROMISES0.
+      eapply split_succeed_wf in PROMISES. des. des_ifs.
+      + ss. des. clarify.
+      + ss. guardH o. des. clarify.
+        esplits; eauto.
+      + esplits; eauto.
+    - des. clarify. erewrite Memory.lower_o; eauto. des_ifs.
+      + ss. des. clarify.
+        eapply lower_succeed_wf in PROMISES. des. clarify.
+      + esplits; eauto.
+    - clarify.
+  Qed.
 
-Lemma caps_collapsing_ident3 L mem maxts loc ts fts
-      (RESERVEWF : memory_reserve_wf mem)
-      (INHABITED : Memory.inhabited mem)
-      (MAX: Memory.max_full_ts mem loc maxts)
-      (TS: Time.lt fts maxts)
-      (MAP: (caps_collapsing L mem) loc ts fts)
-  :
-    ts = fts.
-Proof.
-  inv MAP; eauto.
-  exploit Memory.max_full_ts_inj.
-  { eapply FULL. }
-  { eapply MAX. }
-  i. clarify. exfalso. eapply Time.lt_strorder; eauto.
-Qed.
+  Lemma remove_not_cacncel_reserves_same prom0 loc from to val released prom1
+        (REMOVE: Memory.remove prom0 loc from to (Message.full val released) prom1)
+        loc0 to0 from0
+        (GET: Memory.get loc0 to0 prom0 = Some (from0, Message.reserve))
+    :
+      exists from1,
+        Memory.get loc0 to0 prom1 = Some (from1, Message.reserve).
+  Proof.
+    dup REMOVE. eapply Memory.remove_get0 in REMOVE. des.
+    eapply Memory.remove_o in REMOVE0.
+    instantiate (1:=to0) in REMOVE0.
+    instantiate (1:=loc0) in REMOVE0. des_ifs.
+    - ss. des. clarify.
+    - esplits. etrans; eauto.
+  Qed.
 
-Lemma caps_collapsing_timemap L mem tm
-      (INHABITED: Memory.inhabited mem)
-      (TM: Memory.closed_timemap tm mem)
-  :
-    timemap_map (caps_collapsing L mem) tm tm.
-Proof.
-  exploit Memory.max_full_timemap_exists; eauto. intros [maxmap MAX].
-  eapply identity_mapped_view.
-  - eapply Memory.max_full_timemap_spec; eauto.
-  - i. eapply caps_collapsing_ident; eauto.
-Qed.
+  Lemma step_not_cancel_reserves_same P lang e th0 th1
+        (STEPS: (@pred_step P lang) e th0 th1)
+        (PRED: P <1= (promise_free /1\ (fun e => ~ is_cancel e)))
+        loc to from
+        (GET: Memory.get loc to th0.(Thread.local).(Local.promises) = Some (from, Message.reserve))
+    :
+      exists from',
+        Memory.get loc to th1.(Thread.local).(Local.promises) = Some (from', Message.reserve).
+  Proof.
+    inv STEPS. eapply PRED in SAT. inv STEP. inv STEP0.
+    - inv STEP. des. ss. inv LOCAL.
+      eapply promise_not_cacncel_reserves_same; eauto.
+      ii. clarify.
+    - inv STEP. inv LOCAL; ss.
+      + esplits; eauto.
+      + inv LOCAL0. esplits; eauto.
+      + inv LOCAL0. inv WRITE. ss.
+        eapply promise_not_cacncel_reserves_same in GET; cycle 1; eauto.
+        { ii. clarify. inv PROMISE. clarify. } des.
+        eapply remove_not_cacncel_reserves_same in GET; cycle 1; eauto.
+      + inv LOCAL2. inv WRITE. ss. inv LOCAL1. ss.
+        eapply promise_not_cacncel_reserves_same in GET; cycle 1; eauto.
+        { ii. clarify. inv PROMISE. clarify. } des.
+        eapply remove_not_cacncel_reserves_same in GET; cycle 1; eauto.
+      + inv LOCAL0. esplits; eauto.
+      + inv LOCAL0. esplits; eauto.
+      + inv LOCAL0. esplits; eauto.
+  Qed.
 
-Lemma caps_collapsing_view L mem vw
-      (INHABITED: Memory.inhabited mem)
-      (VW: Memory.closed_view vw mem)
-  :
-    view_map (caps_collapsing L mem) vw vw.
-Proof.
-  inv VW. econs.
-  - eapply caps_collapsing_timemap; eauto.
-  - eapply caps_collapsing_timemap; eauto.
-Qed.
+  Lemma steps_not_cancel_reserves_same P lang th0 th1
+        (STEPS: rtc (tau (@pred_step P lang)) th0 th1)
+        (PRED: P <1= (promise_free /1\ (fun e => ~ is_cancel e)))
+        loc to from
+        (GET: Memory.get loc to th0.(Thread.local).(Local.promises) = Some (from, Message.reserve))
+    :
+      exists from',
+        Memory.get loc to th1.(Thread.local).(Local.promises) = Some (from', Message.reserve).
+  Proof.
+    ginduction STEPS; i.
+    - esplits; eauto.
+    - inv H. exploit step_not_cancel_reserves_same; eauto. i. des.
+      exploit IHSTEPS; eauto.
+  Qed.
 
-Lemma caps_collapsing_opt_view L mem vw
-      (INHABITED: Memory.inhabited mem)
-      (VW: Memory.closed_opt_view vw mem)
-  :
-    opt_view_map (caps_collapsing L mem) vw vw.
-Proof.
-  inv VW; econs.
-  eapply caps_collapsing_view; eauto.
-Qed.
+  Lemma cancel_promises_decrease P lang e th0 th1
+        (STEP: (@pred_step P lang) e th0 th1)
+        (PRED: P <1= is_cancel)
+    :
+      Memory.le th1.(Thread.local).(Local.promises) th0.(Thread.local).(Local.promises).
+  Proof.
+    inv STEP. eapply PRED in SAT. unfold is_cancel in SAT. des_ifs.
+    inv STEP0. inv STEP; inv STEP0; ss.
+    - inv LOCAL. inv PROMISE; ss.
+      ii. erewrite Memory.remove_o in LHS; eauto. des_ifs.
+    - inv LOCAL.
+  Qed.
 
-Lemma caps_collapsing_message L mem msg
-      (INHABITED: Memory.inhabited mem)
-      (MSG: Memory.closed_message msg mem)
-  :
-    msg_map (caps_collapsing L mem) msg msg.
-Proof.
-  inv MSG; econs.
-  eapply caps_collapsing_opt_view; eauto.
-Qed.
-
-Lemma caps_collapsing_tview L mem vw
-      (INHABITED: Memory.inhabited mem)
-      (VW: TView.closed vw mem)
-  :
-    tview_map (caps_collapsing L mem) vw vw.
-Proof.
-  inv VW. econs.
-  - i. eapply caps_collapsing_view; eauto.
-  - eapply caps_collapsing_view; eauto.
-  - eapply caps_collapsing_view; eauto.
-Qed.
-
-Lemma memory_cap_message_closed prom mem0 mem1
-      (CLOSED: Memory.closed mem0)
-      (CAP: Memory.cap prom mem0 mem1)
-      loc to from msg
-      (GET: Memory.get loc to mem1 = Some (from, msg))
-  :
-    Memory.closed_message msg mem0.
-Proof.
-  eapply Memory.cap_inv in GET; eauto. des.
-  - eapply CLOSED in GET. des; auto.
-  - clarify.
-  - clarify. econs. econs.
-    eapply Memory.max_full_view_closed; eauto.
-Qed.
-
-Lemma caps_collapsing_promises (L: Loc.t -> Prop) mem prom
-      (MLE: Memory.le prom mem)
-      (CLOSED: Memory.closed mem)
-      (RESERVEWF: memory_reserve_wf mem)
-      (COLLAPSABLE: collapsable_cap L prom mem)
-  :
-    promises_map (caps_collapsing L mem) prom prom.
-Proof.
-  exploit Memory.max_full_timemap_exists; eauto.
-  { inv CLOSED. eauto. }
-  intros [tm MAX].
-  dup CLOSED. inv CLOSED0. econs.
-  - i. dup GET. eapply MLE in GET0. eapply CLOSED1 in GET0. des.
-    exists to, from, msg.
-    destruct (classic (L loc)).
-    + dup GET. eapply MLE in GET0.
-      eapply not_latest_reserve_le_max_full_ts in GET0; eauto.
-      eapply or_strengthen in GET0. des; clarify.
-      * esplits; eauto.
-        { ii. unfold collapsed in *. des.
-          eapply caps_collapsing_ident2 in MAP1; eauto; cycle 1.
-          eapply caps_collapsing_ident2 in MAP0; eauto; cycle 1.
-          { etrans; eauto. left. auto. } clarify.
-          eapply Time.lt_strorder; eauto. }
-        { econs 2; eauto. }
-        { eapply caps_collapsing_message; eauto. }
-      * exfalso. exploit COLLAPSABLE; eauto.
-    + splits; auto.
-      * ii. unfold collapsed in *. des.
-        inv MAP0; clarify. inv MAP1; clarify.
-        eapply Time.lt_strorder. eauto.
-      * econs 1; eauto.
-      * eapply caps_collapsing_message; eauto.
-  - i. exists fto, ffrom, fmsg.
-    destruct (classic (L loc)).
-    + dup GET. eapply MLE in GET.
-      eapply not_latest_reserve_le_max_full_ts in GET; eauto.
-      des; clarify.
-      * splits; auto.
-        { eapply caps_collapsing_ident; eauto. }
-        { eapply caps_collapsing_ident; eauto.
-          etrans; eauto.
-          eapply memory_get_ts_strong in GET0. des; clarify.
-          { refl. }
-          { left. auto. } }
-      * exfalso. exploit COLLAPSABLE; eauto.
-    + splits; auto.
-      * econs 1; eauto.
-      * econs 1; eauto.
-Qed.
-
-Lemma caps_collapsing_memory' (L0 L1: Loc.t -> Prop)
-      mem0 mem1 mem2 mem3 prom
-      (MLE: Memory.le prom mem0)
-      (CLOSED: Memory.closed mem0)
-      (RESERVEWF0: memory_reserve_wf mem0)
-      (RESERVEWF1: Memory.reserve_wf prom mem0)
-      (COLLAPSABLE0: collapsable_cap L0 prom mem0)
-      (COLLAPSABLE1: collapsable_cap L1 prom mem0)
-      (CAP: Memory.cap prom mem0 mem1)
-      (FORGET0: forget_memory (collapsing_latest_reserves_times L0 mem0 \2/ collapsing_caps_times L0 mem0 mem1) mem2 mem1)
-      (FORGET1: forget_memory (collapsing_latest_reserves_times L1 mem0 \2/ collapsing_caps_times L1 mem0 mem1) mem3 mem2)
-  :
-    memory_map (caps_collapsing L1 mem0) mem2 mem3.
-Proof.
-  exploit Memory.max_full_timemap_exists; eauto.
-  { inv CLOSED. eauto. }
-  intros [tm MAX].
-  dup FORGET0. inv FORGET0. dup FORGET1. inv FORGET1.
-  dup CLOSED. inv CLOSED0. econs.
-  - i. dup GET. eapply forget_memory_get in GET0; eauto. des.
-    destruct (classic (L1 loc)).
-    + destruct (classic ((collapsing_latest_reserves_times L1 mem0 \2/ collapsing_caps_times L1 mem0 mem1) loc to)).
-      * des.
-        { inv H0. inv H1. des. clarify.
-          dup RESERVE. eapply Memory.cap_le in RESERVE0; eauto; [|refl]. clarify.
-          replace from with (tm loc) in *; cycle 1.
-          { eapply Memory.max_full_ts_inj; eauto.
-            eapply max_ts_reserve_from_full_ts; eauto. }
-          dup RESERVE0. eapply RESERVEWF0 in RESERVE. des.
-          eapply Memory.cap_le in RESERVE; eauto. refl.
-        }
-        { inv H0. inv H1. des.
-          dup CAP0. eapply caps_max_view in CAP0; eauto. des. clarify.
-          unfold caps in CAP1. des. clarify.
-          inv VAL.
-          exploit Memory.max_full_ts_inj.
-          { eapply MAX0. }
-          { eapply MAX. } i. clarify.
-          exploit Memory.max_full_ts_spec; eauto. i. des. clarify. right.
-          exists (tm loc), from, (Message.full val (Some (View.mk tm tm))), (Message.full val released).
-          splits.
-          - econs 3; eauto.
-            { eapply TimeFacts.le_lt_lt.
-              - eapply max_full_ts_le_max_ts; eauto.
-              - eapply DenseOrder.DenseOrder.incr_spec. }
-            { refl. }
-          - eapply caps_collapsing_message; eauto. econs. econs.
-            eapply Memory.max_full_view_closed. econs; eauto.
-          - econs. eapply CLOSED1 in GET3. des. inv MSG_CLOSED.
-            inv CLOSED0; eauto. inv CLOSED2. econs. econs; ss.
-            + eapply Memory.max_full_timemap_spec; eauto.
-            + eapply Memory.max_full_timemap_spec; eauto.
-          - erewrite COMPLETE0; eauto.
-            + erewrite COMPLETE; eauto.
-              * eapply Memory.cap_le in GET3; eauto. refl.
-              * eapply max_full_ts_not_collapsed; eauto.
-            + eapply max_full_ts_not_collapsed; eauto. }
-      * apply not_or_and in H0. des.
-        assert (TS: Time.le to (tm loc)).
-        { dup GET1. eapply Memory.cap_inv in GET1; eauto. des; clarify.
-          - dup GET1. eapply not_latest_reserve_le_max_full_ts in GET1; eauto.
-            des; clarify. exfalso. eapply H0. econs; eauto. econs; eauto.
-          - inv GET2. dup GET5. eapply not_latest_reserve_le_max_full_ts in GET5; eauto.
-            des; clarify.
-            + eapply memory_get_ts_le in GET2. etrans; eauto.
-            + refl.
-          - exfalso. eapply H1. econs; eauto. econs; eauto.
-            esplits; eauto. econs; eauto. }
-        right. exists to, from, msg, msg. splits; auto.
-        { econs 2; eauto. }
-        { eapply caps_collapsing_message; eauto.
-          eapply memory_cap_message_closed; eauto. }
-        { refl. }
-        { erewrite COMPLETE0; eauto. ii. des; clarify. }
-    + right. exists to, from, msg, msg. esplits; eauto.
-      * econs 1; eauto.
-      * eapply caps_collapsing_message; eauto.
-        eapply memory_cap_message_closed in GET1; eauto.
-      * refl.
-      * erewrite COMPLETE0; eauto. ii. des.
-        { inv H0. inv H1. des. clarify. }
-        { inv H0. inv H1. des. clarify. }
-  - i. dup GET. eapply forget_memory_get in GET0; eauto. des.
-    apply not_or_and in NOT. des.
-    exists fto, ffrom, fmsg. destruct (classic (L1 loc)).
-    + assert (TS: Time.le fto (tm loc)).
-      { dup GET1. eapply forget_memory_get in GET1; eauto. des.
-        dup GET2. eapply Memory.cap_inv in GET2; eauto. des; clarify.
-        - dup GET2. eapply not_latest_reserve_le_max_full_ts in GET2; eauto.
-          des; clarify. exfalso. eapply NOT. econs; eauto. econs; eauto.
-        - inv GET3. dup GET6. eapply not_latest_reserve_le_max_full_ts in GET6; eauto.
-          des; clarify.
-          + eapply memory_get_ts_le in GET3. etrans; eauto.
-          + refl.
-        - exfalso. eapply NOT0. econs; eauto. econs; eauto.
-          esplits; eauto. econs; eauto. }
-      splits; auto.
-      * econs 2; eauto.
-      * econs 2; eauto. etrans; eauto.
-        eapply memory_get_ts_le; eauto.
-    + splits; auto.
-      * econs 1; eauto.
-      * econs 1; eauto.
-Qed.
-
-(* TODO: move it to DRF_PF0 *)
-Lemma bot_forget P mem0
-      (BOT: P <2= bot2)
-  :
-    forget_memory P mem0 mem0.
-Proof.
-  econs; eauto. i. eapply BOT in PROMS. clarify.
-Qed.
-
-Lemma caps_collapsing_memory
-      mem0 mem1 mem2 prom (L: Loc.t -> Prop)
-      (MLE: Memory.le prom mem0)
-      (CLOSED: Memory.closed mem0)
-      (RESERVEWF0: memory_reserve_wf mem0)
-      (RESERVEWF1: Memory.reserve_wf prom mem0)
-      (COLLAPSABLE: collapsable_cap L prom mem0)
-      (CAP: Memory.cap prom mem0 mem1)
-      (FORGET: forget_memory (collapsing_latest_reserves_times L mem0 \2/ collapsing_caps_times L mem0 mem1) mem2 mem1)
-  :
-    memory_map (caps_collapsing L mem0) mem1 mem2.
-Proof.
-  eapply (@caps_collapsing_memory' bot1); eauto.
-  - ii. clarify.
-  - eapply bot_forget. i.
-    unfold collapsing_latest_reserves_times, collapsing_caps_times,
-    collapsing_latest_reserves, collapsing_caps in PR. des; clarify.
-Qed.
-
-(* Definition memory_last_reserves (prom mem: Memory.t) := (fun loc => Memory.latest_reserve loc prom mem). *)
-
-Definition pf_consistent_drf' lang (e0:Thread.t lang): Prop :=
-  let L := (fun loc => Memory.latest_reserve loc e0.(Thread.local).(Local.promises) e0.(Thread.memory)) in
-  forall mem1 mem2
-         (CAP: Memory.cap e0.(Thread.local).(Local.promises) e0.(Thread.memory) mem1)
-         (FORGET: forget_memory (collapsing_latest_reserves_times L e0.(Thread.memory) \2/ collapsing_caps_times L e0.(Thread.memory) mem1) mem2 mem1),
-  exists e1,
-    (<<STEPS0: rtc (tau (@pred_step is_cancel lang)) (Thread.mk _ e0.(Thread.state) e0.(Thread.local) TimeMap.bot mem2) e1>>) /\
-    (<<NORESERVE: no_reserves e1.(Thread.local).(Local.promises)>>) /\
-    exists e2,
-      (<<STEPS1: rtc (tau (@pred_step ((promise_free /1\ (fun e => ~ is_cancel e) /1\ no_acq_update_msgs ((fun loc to => L loc) /2\ Memory.max_full_ts e0.(Thread.memory))) /1\ no_sc) lang)) e1 e2>>) /\
-      (__guard__((<<FAILURE: Local.failure_step e2.(Thread.local)>>) \/
-                 (<<PROMISES: e2.(Thread.local).(Local.promises) = Memory.bot>>))).
-
-Lemma caps_collapsing_collapsable_unwritable L prom mem0 mem1
-      (MLE: Memory.le prom mem0)
-      (RESERVEWF : memory_reserve_wf mem0)
-      (INHABITED : Memory.inhabited mem0)
-      (COLLAPSABLE: collapsable_cap L prom mem0)
-      (CAP: Memory.cap prom mem0 mem1)
-  :
-    collapsable_unwritable (caps_collapsing L mem0) prom mem1.
-Proof.
-  ii. des. unfold collapsed in *. des. inv ITV. ss.
-  inv MAP0; inv MAP1; clarify.
-  - exfalso; eapply Time.lt_strorder; eapply TimeFacts.lt_le_lt; eauto.
-  - exfalso; eapply Time.lt_strorder; eapply TimeFacts.lt_le_lt; eauto.
-  - exploit Memory.max_full_ts_inj; [apply FULL|apply FULL0|i; clarify].
-    inv CAP. destruct (Time.le_lt_dec t (Memory.max_ts loc mem0)).
-    + exploit max_full_ts_max_ts; eauto. i. des; clarify.
-      * clear - FROM l.
-        exfalso; eapply Time.lt_strorder; eapply TimeFacts.lt_le_lt; eauto.
-      * econs; eauto.
-        { econs; eauto.
-          destruct (Memory.get loc (Memory.max_ts loc mem0) prom) eqn:GETPROM; eauto.
-          exfalso. destruct p as [from []].
-          - eapply MLE in GETPROM. clarify.
-          - eapply COLLAPSABLE in GETPROM; eauto. }
-        { econs; ss. }
-    + exploit Memory.latest_val_exists; eauto. i. des.
-      exploit Memory.max_full_view_exists; eauto. i. des.
-      exploit BACK; eauto.
-      { instantiate (1:=loc). unfold Memory.latest_reserve. des_ifs.
-        eapply COLLAPSABLE in Heq; eauto. }
-      i. econs; eauto.
-      * econs; eauto.
-        destruct (Memory.get loc (Time.incr (Memory.max_ts loc mem0)) prom) eqn:GETPROM; eauto.
-        exfalso. destruct p as [from msg].
-        eapply MLE in GETPROM.
-        eapply Memory.max_ts_spec in GETPROM; eauto. des.
-        exfalso; eapply Time.lt_strorder; eapply TimeFacts.lt_le_lt; eauto.
-      * econs; eauto.
-  - clear - FROM TO. exfalso; eapply Time.lt_strorder; eapply TimeFacts.lt_le_lt; eauto.
-  - exploit Memory.max_full_ts_inj; [apply FULL|apply FULL0|i; clarify].
-    exfalso; eapply Time.lt_strorder; eapply TimeFacts.le_lt_lt.
-    { eapply TO. }
-    etrans; eauto.
-  - exploit Memory.max_full_ts_inj; [apply FULL|apply FULL0|i; clarify].
-    inv CAP. destruct (Time.le_lt_dec t (Memory.max_ts loc mem0)).
-    + exploit max_full_ts_max_ts; eauto. i. des; clarify.
-      * clear - FROM TS0 l.
-        exfalso; eapply Time.lt_strorder; eapply TimeFacts.lt_le_lt; eauto.
-        etrans; eauto. left. auto.
-      * econs; eauto.
-        { econs; eauto.
-          destruct (Memory.get loc (Memory.max_ts loc mem0) prom) eqn:GETPROM; eauto.
-          exfalso. destruct p as [from []].
-          - eapply MLE in GETPROM. clarify.
-          - eapply COLLAPSABLE in GETPROM; eauto. }
-        { econs; ss. clear - FROM TS0. etrans; eauto. }
-    + exploit Memory.latest_val_exists; eauto. i. des.
-      exploit Memory.max_full_view_exists; eauto. i. des.
-      exploit BACK; eauto.
-      { instantiate (1:=loc). unfold Memory.latest_reserve. des_ifs.
-        eapply COLLAPSABLE in Heq; eauto. }
-      i. econs; eauto.
-      * econs; eauto.
-        destruct (Memory.get loc (Time.incr (Memory.max_ts loc mem0)) prom) eqn:GETPROM; eauto.
-        exfalso. destruct p as [from msg].
-        eapply MLE in GETPROM.
-        eapply Memory.max_ts_spec in GETPROM; eauto. des.
-        exfalso; eapply Time.lt_strorder; eapply TimeFacts.lt_le_lt; eauto.
-      * econs; eauto.
-  - exfalso; eapply Time.lt_strorder; eapply TimeFacts.le_lt_lt; eauto.
-  - clear - FROM TO. exfalso; eapply Time.lt_strorder; eapply TimeFacts.lt_le_lt; eauto.
-  - exfalso; eapply Time.lt_strorder; eapply TimeFacts.le_lt_lt.
-    { eapply TS1. }
-    etrans; eauto.
-  - clear - FROM TO. exfalso; eapply Time.lt_strorder; eapply TimeFacts.lt_le_lt; eauto.
-Qed.
-
-Lemma caps_collapsing_mapping_map_le L prom mem0 mem1
-      (COLLAPSABLE: collapsable_cap L prom mem0)
-      (CAP: Memory.cap prom mem0 mem1)
-  :
-    mapping_map_le (caps_collapsing L mem0).
-Proof.
-  ii. inv MAP0; inv MAP1; clarify.
-  - exploit Memory.max_full_ts_inj; [apply FULL|apply FULL0|i; clarify].
-  - etrans; eauto. left. auto.
-  - exploit Memory.max_full_ts_inj; [apply FULL|apply FULL0|i; clarify]. refl.
-  - etrans; eauto. left. auto.
-  - exfalso; eapply Time.lt_strorder; eapply TimeFacts.lt_le_lt.
-    { eapply TLE. }
-    etrans; eauto.
-Qed.
-
-Lemma caps_collapsing_mapping_map_bot L prom mem0 mem1
-      (COLLAPSABLE: collapsable_cap L prom mem0)
-      (INHABITED: Memory.inhabited mem0)
-      (CAP: Memory.cap prom mem0 mem1)
-  :
-    mapping_map_bot (caps_collapsing L mem0).
-Proof.
-  ii. destruct (classic (L loc)).
-  - exploit Memory.max_full_ts_exists; eauto. i. des.
-    econs 2; eauto. eapply Time.bot_spec.
-  - econs 1; eauto.
-Qed.
-
-Lemma caps_collapsing_mapping_map_eq L prom mem0 mem1
-      (COLLAPSABLE: collapsable_cap L prom mem0)
-      (CAP: Memory.cap prom mem0 mem1)
-  :
-    mapping_map_eq (caps_collapsing L mem0).
-Proof.
-  ii. inv MAP0; inv MAP1; clarify.
-  - exploit Memory.max_full_ts_inj; [apply FULL|apply FULL0|i; clarify].
-    exfalso; eapply Time.lt_strorder; eapply TimeFacts.lt_le_lt; eauto.
-  - exploit Memory.max_full_ts_inj; [apply FULL|apply FULL0|i; clarify].
-    exfalso; eapply Time.lt_strorder; eapply TimeFacts.le_lt_lt; eauto.
-  - exploit Memory.max_full_ts_inj; [apply FULL|apply FULL0|i; clarify].
-  - exfalso; eapply Time.lt_strorder; eapply TimeFacts.lt_le_lt; eauto.
-  - clear - TLE TS1. exfalso; eapply Time.lt_strorder; eapply TimeFacts.lt_le_lt; eauto.
-Qed.
-
-Lemma caps_collapsing_total L mem0 loc to
-      (INHABITED: Memory.inhabited mem0)
-  :
-    exists fto,
-      <<MAP: caps_collapsing L mem0 loc to fto >>.
-Proof.
-  destruct (classic (L loc)).
-  - exploit Memory.max_full_ts_exists; eauto. i. des.
-    destruct (Time.le_lt_dec to ts).
-    { eexists. econs 2; eauto. }
-    destruct (Time.le_lt_dec to (Time.incr (Memory.max_ts loc mem0))).
-    { eexists. econs 3; eauto. }
-    { eexists. econs 4; eauto. }
-  - eexists. econs 1; eauto.
-Qed.
-
-Lemma caps_collapsing_mappable_time_always L mem0
-      (INHABITED: Memory.inhabited mem0)
-      loc to
-  :
-    mappable_time (caps_collapsing L mem0) loc to.
-Proof.
-  eapply caps_collapsing_total; eauto.
-Qed.
-
-Lemma caps_collapsing_mappable_event_always L mem0
-      (INHABITED: Memory.inhabited mem0)
-      e
-  :
-    mappable_evt (caps_collapsing L mem0) e.
-Proof.
-  destruct e; ss; split; (apply caps_collapsing_mappable_time_always; auto).
-Qed.
-
-Lemma collapsing_caps_forget_closed
-      mem0 mem1 mem2 prom (L: Loc.t -> Prop)
-      (CLOSED: Memory.closed mem0)
-      (CAP: Memory.cap prom mem0 mem2)
-      (FORGET: forget_memory (collapsing_latest_reserves_times L mem0 \2/ collapsing_caps_times L mem0 mem2) mem1 mem2)
-  :
-    Memory.closed mem1.
-Proof.
-  hexploit collapsing_caps_forget_le; eauto. intros MLE.
-  inv CLOSED.
-  econs.
-  - ii. eapply forget_memory_get in MSG; eauto. des.
-    eapply Memory.cap_inv in GET; try apply CAP; eauto. des; clarify.
-    + eapply CLOSED0 in GET; eauto. des. splits; auto.
-      eapply memory_concrete_le_closed_msg; eauto.
-    + split; auto. econs.
-    + splits; auto.
-      * econs; eauto. econs. eapply Memory.max_full_view_wf; eauto.
-      * econs; eauto. ss. inv GET4. ss. etrans.
-        { eapply max_full_ts_le_max_ts; eauto. }
-        { left. eapply Time.incr_spec. }
-      * eapply memory_concrete_le_closed_msg; eauto.
-        econs; eauto. econs.
-        eapply Memory.max_full_view_closed; eauto.
-  - ii. eauto.
-Qed.
-
-Lemma pf_consistent_pf_consistent_drf' lang (th: Thread.t lang)
-      (WF: Local.wf th.(Thread.local) th.(Thread.memory))
-      (MEM: Memory.closed th.(Thread.memory))
-      (CONSISTENT: pf_consistent_strong th)
-      (RESERVEWF: memory_reserve_wf (Thread.memory th))
-  :
-    pf_consistent_drf' th.
-Proof.
-  assert (INHABITED: Memory.inhabited th.(Thread.memory)).
-  { inv MEM. auto. }
-  ii.
-  set (L:=fun loc : Loc.t =>
-                      Memory.latest_reserve loc (Local.promises (Thread.local th)) (Thread.memory th)).
-  assert (COLLAPSABLE: collapsable_cap L (Local.promises (Thread.local th)) (Thread.memory th)).
-  { ii. clarify. unfold L, Memory.latest_reserve in SAT.
-    rewrite GET in SAT. clarify. }
-  assert (MAPLE: mapping_map_le (caps_collapsing L th.(Thread.memory))).
-  { eapply caps_collapsing_mapping_map_le; eauto. }
-  assert (MAPBOT: mapping_map_bot (caps_collapsing L th.(Thread.memory))).
-  { eapply caps_collapsing_mapping_map_bot; eauto. }
-  assert (MAPEQ: mapping_map_eq (caps_collapsing L th.(Thread.memory))).
-  { eapply caps_collapsing_mapping_map_eq; eauto. }
-  assert (CONCRETELE: memory_concrete_le th.(Thread.memory) mem2).
-  { eapply collapsing_caps_forget_le; eauto. }
-
-  exploit CONSISTENT; eauto. i. des.
-
-  assert (WFTGT: Local.wf (Thread.local th) mem1).
-  { eapply Local.cap_wf; eauto. }
-  assert (CLOSEDTGT: Memory.closed mem1).
-  { eapply Memory.cap_closed; eauto. }
-  assert (CLOSEDSRC: Memory.closed mem2).
-  { eapply collapsing_caps_forget_closed; cycle 1; eauto. }
-  assert (LCWFSRC: Local.wf th.(Thread.local) mem2).
-  { eapply memory_concrete_le_local_wf; eauto. inv WF.
-    eapply collapsing_caps_forget_prom_le; eauto. }
-
-  assert (SCSRC: Memory.closed_timemap TimeMap.bot mem2).
-  { eapply Memory.closed_timemap_bot; eauto. }
-  assert (SCTGT: Memory.closed_timemap TimeMap.bot mem1).
-  { eapply Memory.closed_timemap_bot; eauto.
-    ii. eapply Memory.cap_le; eauto. refl. }
-  assert (UNWRITABLE: collapsable_unwritable
-                        (caps_collapsing L (Thread.memory th))
-                        (Local.promises (Thread.local th)) mem1).
-  { inv WF. eapply caps_collapsing_collapsable_unwritable; eauto. }
-
-  destruct e1.
-  hexploit (@steps_map (caps_collapsing L (Thread.memory th))); try apply STEPS0; auto; eauto.
-  { i. eapply caps_collapsing_mappable_event_always; eauto. }
-  { econs.
+  Lemma cancels_promises_decrease P lang th0 th1
+        (STEP: rtc (tau (@pred_step P lang)) th0 th1)
+        (PRED: P <1= is_cancel)
+    :
+      Memory.le th1.(Thread.local).(Local.promises) th0.(Thread.local).(Local.promises).
+  Proof.
+    ginduction STEP.
     - refl.
-    - eapply caps_collapsing_tview; eauto. inv WF. eauto.
-    - eapply caps_collapsing_promises; eauto. inv WF. eauto. }
-  { inv WF. eapply caps_collapsing_memory; try apply FORGET; eauto. }
-  { eapply timemap_bot_map; eauto. }
-  { refl. }
-  { instantiate (1:=is_cancel). ii. inv REL; ss. inv KIND; ss. }
-  i. des.
+    - etrans; eauto. inv H.
+      eapply cancel_promises_decrease; eauto.
+  Qed.
 
-  exploit Thread.rtc_tau_step_future.
-  { eapply thread_steps_pred_steps. eapply STEPS0. } all: eauto. i. des. ss.
-  exploit Thread.rtc_tau_step_future.
-  { eapply thread_steps_pred_steps. eapply STEP. } all: eauto. i. des. ss.
+End CANCEL.
 
-  destruct e2.
-  eapply steps_write_not_in in STEPS1; cycle 1.
-  { inv WF2. ss. }
-  eapply steps_wf_event in STEPS1; cycle 1.
-  { inv CLOSED2. ss. }
+Section CAP.
 
-  hexploit (@steps_map (caps_collapsing L (Thread.memory th))); try apply STEPS1; auto; eauto.
-  { i. eapply caps_collapsing_mappable_event_always; eauto. }
-  { eapply collapsable_unwritable_steps in STEPS0; eauto. }
-  { instantiate (1:=(promise_free /1\ (fun e => ~ is_cancel e) /1\ no_acq_update_msgs ((fun loc to => L loc) /2\ Memory.max_full_ts th.(Thread.memory))) /1\ no_sc).
-    ss. ii. des. inv REL; splits; ss; eauto.
-    - inv KIND; ss. inv MSG0; ss. inv MSG; ss. inv MAP0; ss.
-    - inv KIND; ss.
-    - ii. des.
-      specialize (SAT1 (Time.meet to (Time.incr (Memory.max_ts loc (Thread.memory th))))).
-      inv FROM.
-      + clarify.
-      + exploit Memory.max_full_ts_inj; [apply SAT6|apply FULL|i; clarify].
-        assert (TS: Time.lt max (Time.incr (Memory.max_ts loc (Thread.memory th)))).
-        { eapply TimeFacts.le_lt_lt.
-          { eapply max_full_ts_le_max_ts; eauto. }
-          { eapply Time.incr_spec. } }
-        assert (UNWRITABLE0: unwritable memory (Local.promises local) loc (Time.meet to (Time.incr (Memory.max_ts loc (Thread.memory th))))).
-        { exploit rtc_unwritable_increase; [| |].
-          - eapply thread_steps_pred_steps. eapply STEPS0.
-          - ss. eapply UNWRITABLE.
-            eexists max, (Time.incr (Memory.max_ts loc (Thread.memory th))). splits; eauto.
-            + eexists. splits.
-              * econs 2; eauto.
-              * econs 3; eauto. refl.
-            + instantiate (1:=Time.meet to (Time.incr (Memory.max_ts loc (Thread.memory th)))).
-              unfold Time.meet. des_ifs; econs; ss. refl.
-          - ss. }
-        eapply SAT1; eauto. unfold Time.meet. des_ifs; econs; ss.
-        * refl.
-        * left. auto.
-      + destruct TS1.
-        { assert (TS: Time.lt ffrom (Time.incr (Memory.max_ts loc (Thread.memory th)))).
-          { eapply TimeFacts.le_lt_lt.
-            { eapply max_full_ts_le_max_ts; eauto. }
-            { eapply Time.incr_spec. } }
-          assert (UNWRITABLE0: unwritable memory (Local.promises local) loc (Time.meet to (Time.incr (Memory.max_ts loc (Thread.memory th))))).
-          { exploit rtc_unwritable_increase; [| |].
-            - eapply thread_steps_pred_steps. eapply STEPS0.
-            - ss. eapply UNWRITABLE.
-              eexists ffrom, (Time.incr (Memory.max_ts loc (Thread.memory th))). splits; eauto.
-              + eexists. splits.
-                * econs 2; eauto. refl.
-                * econs 3; eauto. refl.
-              + instantiate (1:=Time.meet to (Time.incr (Memory.max_ts loc (Thread.memory th)))).
-                unfold Time.meet. des_ifs; econs; ss.
-                * transitivity from; auto.
-                * refl.
-            - ss. }
-          eapply SAT1; eauto. unfold Time.meet. des_ifs; econs; ss.
-          * refl.
-          * left. auto. }
-        { unfold Time.eq in *. subst.
-          eapply SAT3; eauto. econs; eauto. inv CAP.
-          hexploit (@Memory.latest_val_exists loc (Thread.memory th)); eauto. i. des.
-          hexploit (@Memory.max_full_view_exists (Thread.memory th)); eauto. i. des.
-          exploit BACK; eauto. i.
-          esplits; eauto. econs; eauto.
-          destruct (Memory.get loc (Time.incr (Memory.max_ts loc (Thread.memory th))) (Thread.memory th)) eqn: GET; auto.
-          exfalso. destruct p.
-          eapply Memory.max_ts_spec in GET. des.
-          eapply Time.lt_strorder. eapply TimeFacts.le_lt_lt.
-          - eapply MAX.
-          - eapply Time.incr_spec. }
-      + exfalso. eapply Time.lt_strorder. eapply TimeFacts.lt_le_lt.
-        { eapply TLE. }
-        etrans.
-        { eapply max_full_ts_le_max_ts; eauto. }
-        { left. eapply Time.incr_spec. }
-  }
-  i. des.
-  esplits; eauto.
-  - ss. inv LOCAL. eapply no_reserves_map; eauto.
-  - ss. unguard. des.
-    + left. econs. inv FAILURE. inv LOCAL0.
-      eapply promise_consistent_mon.
-      { eapply promise_consistent_map; eauto. }
-      { ss. }
-      { ss. }
-    + right. inv LOCAL0. rewrite PROMISES in *.
-      eapply bot_promises_map; eauto.
-Qed.
+  Definition caps (mem0 mem1 : Memory.t) (l : Loc.t) (t from : Time.t) (msg : Message.t) :=
+    (<<GET0: Memory.get l t mem0 = None>>) /\
+    (<<GET1: Memory.get l t mem1 = Some (from, msg)>>).
 
+  Definition caps_loc (mem0 mem1 : Memory.t) (l : Loc.t) (t : Time.t): Prop :=
+    exists from msg, (<<CAPS: caps mem0 mem1 l t from msg>>).
 
-Definition pf_consistent_drf'' lang (e0:Thread.t lang): Prop :=
-  let L := (fun loc => Memory.latest_reserve loc e0.(Thread.local).(Local.promises) e0.(Thread.memory)) in
-  forall mem1 mem2
-         (CAP: Memory.cap e0.(Thread.local).(Local.promises) e0.(Thread.memory) mem1)
-         (FORGET: forget_memory (collapsing_latest_reserves_times L e0.(Thread.memory) \2/ collapsing_caps_times L e0.(Thread.memory) mem1) mem2 mem1),
-  exists e1,
-    (<<STEPS0: rtc (tau (@pred_step ((promise_free /1\ no_acq_update_msgs ((fun loc to => L loc) /2\ Memory.max_full_ts e0.(Thread.memory))) /1\ no_sc) lang)) (Thread.mk _ e0.(Thread.state) e0.(Thread.local) TimeMap.bot mem2) e1>>) /\
-    (__guard__((<<FAILURE: Local.failure_step e1.(Thread.local)>>) \/
-               (<<PROMISES: e1.(Thread.local).(Local.promises) = Memory.bot>>))).
+  Lemma caps_unchangable mem0 prom mem1
+        (MLE: Memory.le prom mem0)
+        (CAP: Memory.cap prom mem0 mem1)
+    :
+      caps mem0 mem1 <4= unchangable mem1 prom.
+  Proof.
+    i. unfold caps in PR. des. inv CAP.
+    econs; eauto. destruct (Memory.get x0 x1 prom) eqn:GET; auto.
+    destruct p. exfalso. eapply MLE in GET. clarify.
+  Qed.
 
+  Lemma caps_concrete_last mem0 prom mem1 tm l t from val released
+        (RESERVE: Memory.reserve_wf prom mem0)
+        (INHABITED: Memory.inhabited mem0)
+        (MAX: Memory.max_full_timemap mem0 tm)
+        (CAP: Memory.cap prom mem0 mem1)
+        (CAPS: caps mem0 mem1 l t from (Message.full val released))
+    :
+      from = Memory.max_ts l mem0.
+  Proof.
+    unfold caps in CAPS. des. inv CAP.
+    exploit COMPLETE; eauto. i. des.
+    destruct (classic (Memory.max_ts l mem0 = from)); eauto. exfalso.
+    set (@cell_elements_least
+           (mem0 l)
+           (fun to => Time.lt from to)). des.
+    + assert (TLE: Time.le from from0).
+      { dup GET. eapply Memory.get_ts in GET. des; clarify.
+        { exfalso. eapply Time.lt_strorder.
+          eapply TimeFacts.lt_le_lt; eauto. eapply Time.bot_spec. }
+        exploit memory_get_from_mon.
+        - eapply x.
+        - eapply GET2.
+        - eauto.
+        - i. des; clarify. }
+      destruct TLE.
+      * exploit MIDDLE; eauto.
+        econs.
+        { eapply x. }
+        { eapply GET. }
+        { eauto. }
+        { i. destruct (Memory.get l ts mem0) eqn: GET2; auto.
+          destruct p. exfalso. dup GET2. eapply LEAST in GET2; eauto.
+          eapply Memory.get_ts in GET. des; clarify.
+          - eapply Time.lt_strorder. eapply TimeFacts.lt_le_lt.
+            eapply SAT. eapply Time.bot_spec.
+          - eapply Time.lt_strorder. eapply TimeFacts.lt_le_lt.
+            eapply GET. etrans; eauto. }
+        { i. exploit memory_get_from_inj.
+          - eapply x1.
+          - eapply GET1.
+          - i. des; clarify. eapply Time.lt_strorder; eauto. }
+      * destruct H0.
+        exploit memory_get_from_inj.
+        { eapply GET1. }
+        { eapply SOUND. eapply GET. }
+        { i. des; clarify.
+          - unfold Memory.get in GET0. clarify.
+          - eapply Time.lt_strorder; eauto. }
+    + exploit Memory.max_ts_spec.
+      { eapply x. } i. des.
+      eapply EMPTY; eauto. destruct MAX0; clarify.
+      exfalso. eauto.
+  Qed.
 
-Lemma pf_consistent_pf_consistent_drf'' lang (th: Thread.t lang)
-      (WF: Local.wf th.(Thread.local) th.(Thread.memory))
-      (MEM: Memory.closed th.(Thread.memory))
-      (CONSISTENT: pf_consistent_drf' th)
-      (RESERVEWF: memory_reserve_wf (Thread.memory th))
+  Lemma caps_max_view mem0 prom mem1 tm l t from val released
+        (RESERVE: Memory.reserve_wf prom mem0)
+        (INHABITED: Memory.inhabited mem0)
+        (MAX: Memory.max_full_timemap mem0 tm)
+        (CAP: Memory.cap prom mem0 mem1)
+        (CAPS: caps mem0 mem1 l t from (Message.full val released))
+    :
+      (<<FROM: from = Memory.max_ts l mem0>>) /\
+      (<<RESERVE: Memory.latest_reserve l prom mem0>>) /\
+      (<<VAL: Memory.latest_val l mem0 val >>) /\
+      (<<RELEASED: released = Some (View.mk tm tm)>>) /\
+      (<<TO: t = Time.incr (Memory.max_ts l mem0)>>).
+  Proof.
+    exploit caps_concrete_last; eauto. i. clarify.
+    unfold caps in CAPS. des. inv CAP.
+    exploit COMPLETE; eauto. i. des.
+    exploit Memory.latest_val_exists; eauto. i. des.
+    exploit BACK; eauto. i.
+    exploit memory_get_from_inj.
+    { eapply x1. }
+    { eapply GET1. } i. des; clarify.
+    - esplits; eauto.
+    - exfalso. eapply Time.lt_strorder. eapply TimeFacts.lt_le_lt.
+      + eapply Time.incr_spec.
+      + erewrite BOT0. eapply Time.bot_spec.
+    - erewrite INHABITED in GET0. clarify.
+  Qed.
+
+End CAP.
+
+Section PROMISEFREE.
+
+  Lemma promise_free_no_promise P lang (th0 th1: Thread.t lang) e
+        (NOPROMISE: th0.(Thread.local).(Local.promises) = Memory.bot)
+        (STEP: pred_step P e th0 th1)
+        (PRED: P <1= promise_free)
   :
-    pf_consistent_drf'' th.
-Proof.
-  ii. exploit CONSISTENT; eauto. i. des.
-  eexists. esplits.
-  - etrans.
-    + eapply pred_step_rtc_mon; try apply STEPS0.
-      i. destruct x1; ss. destruct kind; ss.
-    + eapply pred_step_rtc_mon; try apply STEPS1.
-      i. ss. des. split; auto.
-  - eauto.
-Qed.
+    (<<STEP: pred_step P e th0 th1>>) /\
+    (<<NOPROMISE: th1.(Thread.local).(Local.promises) = Memory.bot>>).
+  Proof.
+    inv STEP. dup SAT. eapply PRED in SAT. inv STEP0. inv STEP.
+    - inv STEP0. inv LOCAL. inv PROMISE; ss; des; clarify.
+      + rewrite NOPROMISE in *.
+        eapply Memory.lower_get0 in PROMISES. des.
+        erewrite Memory.bot_get in *. clarify.
+      + rewrite NOPROMISE in *.
+        eapply Memory.remove_get0 in PROMISES. des.
+        erewrite Memory.bot_get in *. clarify.
+    - inv STEP0. inv LOCAL.
+      + ss. esplits; eauto. econs; eauto. econs; eauto.
+      + ss. esplits; eauto.
+        * econs; eauto. econs; eauto.
+        * inv LOCAL0. ss.
+      + ss. esplits; eauto.
+        * econs; eauto. econs; eauto.
+        * inv LOCAL0. rewrite NOPROMISE in *.
+          exploit memory_write_bot_add; eauto. i. clarify.
+          inv WRITE. inv PROMISE. ss.
+          symmetry. eapply MemoryMerge.MemoryMerge.add_remove; eauto.
+      + ss. esplits; eauto.
+        * econs; eauto. econs; eauto.
+        * inv LOCAL1. inv LOCAL2. rewrite NOPROMISE in *.
+          exploit memory_write_bot_add; eauto. i. clarify.
+          inv WRITE. inv PROMISE. ss.
+          symmetry. eapply MemoryMerge.MemoryMerge.add_remove; eauto.
+      + ss. esplits; eauto.
+        * econs; eauto. econs; eauto.
+        * inv LOCAL0. ss.
+      + ss. esplits; eauto.
+        * econs; eauto. econs; eauto.
+        * inv LOCAL0. ss.
+      + ss. esplits; eauto.
+        * econs; eauto. econs; eauto.
+  Qed.
 
-Inductive latest_other_reserves (prom mem: Memory.t) (loc: Loc.t) (to: Time.t): Prop :=
-| latest_other_reserves_intro
-    from
-    (MAX: to = Memory.max_ts loc mem)
-    (GET: Memory.get loc to mem = Some (from, Message.reserve))
-    (NONE: Memory.get loc to prom = None)
+  Lemma write_promises_decrease prom0 mem0 loc from to val realeased prom1 mem1 kind
+        (WRITE: Memory.write prom0 mem0 loc from to val realeased prom1 mem1 kind)
+    :
+      concrete_promised prom1 <2= concrete_promised prom0.
+  Proof.
+    inv WRITE. inv PROMISE.
+    - exploit MemoryMerge.MemoryMerge.add_remove.
+      + eapply PROMISES.
+      + eapply REMOVE.
+      + i. clarify.
+    - ii. inv PR.
+      erewrite Memory.remove_o in GET; eauto. des_ifs.
+      erewrite Memory.split_o in GET; eauto. des_ifs.
+      + ss; des; clarify.
+      + ss. des; clarify. eapply Memory.split_get0 in PROMISES.
+        des. econs; eauto.
+      + eapply Memory.split_get0 in PROMISES.
+        guardH o. guardH o0. guardH o1. des. econs; eauto.
+    - ii. inv PR.
+      erewrite Memory.remove_o in GET; eauto. des_ifs.
+      erewrite Memory.lower_o in GET; eauto. des_ifs.
+      + ss; des; clarify.
+      + econs; eauto.
+    - clarify.
+  Qed.
+
+  Lemma pf_step_promises_decrease P lang e (th0 th1: Thread.t lang)
+        (STEP: (@pred_step P lang) e th0 th1)
+        (PRED: P <1= promise_free)
+    :
+      concrete_promised (th1.(Thread.local).(Local.promises)) <2=
+      concrete_promised (th0.(Thread.local).(Local.promises)).
+  Proof.
+    i. inv STEP. eapply PRED in SAT. inv STEP0. des. inv STEP.
+    - inv STEP0. ss. inv LOCAL. ss. inv PROMISE; clarify.
+      + inv PR. erewrite Memory.lower_o in GET; eauto. des_ifs.
+        * ss; des. clarify. eapply Memory.lower_get0 in PROMISES.
+          des. econs; eauto.
+        * econs; eauto.
+      + inv PR. erewrite Memory.remove_o in GET; eauto. des_ifs.
+        econs; eauto.
+    - inv STEP0. ss. inv LOCAL; eauto.
+      + inv LOCAL0. ss.
+      + inv LOCAL0. ss. eapply write_promises_decrease; eauto.
+      + inv LOCAL1. inv LOCAL2. ss. eapply write_promises_decrease; eauto.
+      + inv LOCAL0. ss.
+      + inv LOCAL0. ss.
+  Qed.
+
+  Lemma pf_step_rtc_promises_decrease P lang (th0 th1: Thread.t lang)
+        (STEP: rtc (tau (@pred_step P lang)) th0 th1)
+        (PRED: P <1= promise_free)
+    :
+      concrete_promised (th1.(Thread.local).(Local.promises)) <2=
+      concrete_promised (th0.(Thread.local).(Local.promises)).
+  Proof.
+    ginduction STEP; ss.
+    i. eapply IHSTEP in PR; eauto. inv H.
+    eapply pf_step_promises_decrease; eauto.
+  Qed.
+
+End PROMISEFREE.
+
+
+Section PFCONSISTENT.
+
+  Definition pf_consistent_strong lang (e0:Thread.t lang): Prop :=
+    forall mem1 sc1
+           (CAP: Memory.cap e0.(Thread.local).(Local.promises) e0.(Thread.memory) mem1),
+    exists e1,
+      (<<STEPS0: rtc (tau (@pred_step is_cancel lang)) (Thread.mk _ e0.(Thread.state) e0.(Thread.local) sc1 mem1) e1>>) /\
+      (<<NORESERVE: no_reserves e1.(Thread.local).(Local.promises)>>) /\
+      exists e2,
+        (<<STEPS1: rtc (tau (@pred_step ((promise_free /1\ (fun e => ~ is_cancel e) /1\ no_acq_read_msgs (caps_loc e0.(Thread.memory) mem1)) /1\ no_sc) lang)) e1 e2>>) /\
+        (__guard__((<<FAILURE: Local.failure_step e2.(Thread.local)>>) \/
+                   (<<PROMISES: e2.(Thread.local).(Local.promises) = Memory.bot>>))).
+
+  Lemma pf_consistent_pf_consistent_strong lang (th: Thread.t lang)
+        (WF: Local.wf th.(Thread.local) th.(Thread.memory))
+        (MEM: Memory.closed th.(Thread.memory))
+        (CONSISTENT: pf_consistent th)
+    :
+      pf_consistent_strong th.
+  Proof.
+    assert (INHABITED: Memory.inhabited th.(Thread.memory)).
+    { inv MEM. auto. }
+    ii. exploit Memory.max_full_timemap_exists; eauto. intros MAX. des.
+    ii. exploit Memory.max_full_timemap_exists.
+    { eapply le_inhabited; eauto. eapply Memory.cap_le; eauto. refl. }
+    i. des. exploit CONSISTENT; eauto. i.
+
+    assert (exists e2,
+               (<<STEPS: rtc (tau (Thread.step true))
+                             (Thread.mk _ (Thread.state th) (Thread.local th)
+                                        tm0 mem1) e2 >>) /\
+               (<<NORESERVES: no_reserves e2.(Thread.local).(Local.promises)>>) /\
+               (__guard__ ((exists e3, (<< FAILURE: Thread.step true ThreadEvent.failure e2 e3 >>)) \/
+                           (<<PROMISES: Local.promises (Thread.local e2) = Memory.bot >>)))).
+    { des.
+      - exploit Thread.rtc_tau_step_future.
+        + eapply rtc_implies; [|apply STEPS].
+          i. inv PR. econs; eauto. econs; eauto.
+        + ss. eapply Local.cap_wf; eauto.
+        + ss. eapply Memory.max_full_timemap_closed; eauto.
+        + ss. eapply Memory.cap_closed; eauto.
+        + i. des.
+          destruct e2. destruct local. inv WF2. ss.
+          exploit reserves_cancelable; eauto. i. des.
+          esplits.
+          * etrans.
+            { eapply STEPS. }
+            { eapply rtc_implies; [|apply STEPS0].
+              i. inv PR. inv TSTEP. inv STEP.
+              unfold is_cancel in SAT. des_ifs.
+              inv STEP0; inv STEP.
+              - econs; eauto. econs; eauto. econs; eauto.
+              - inv LOCAL. }
+          * ss.
+          * left. inv FAILURE; inv STEP. inv LOCAL. inv LOCAL0.
+            exists (Thread.mk _ st2 (Local.mk tview proms1) sc2 mem0).
+            ss. econs 2. econs; eauto. econs; eauto. econs; eauto.
+            eapply cancels_promises_decrease in STEPS0; auto. ss.
+            ii. eapply CONSISTENT0; eauto.
+      - unguard. esplits; eauto. rewrite PROMISES. ii.
+        rewrite Memory.bot_get in GET. clarify. }
+
+    clear x. des.
+    eapply pf_step_promise_free_step_rtc in STEPS.
+    eapply pf_steps_cancels_not_cancels in STEPS; cycle 1.
+    { ss. eapply Local.cap_wf; eauto. }
+    { ss. eapply Memory.cap_closed; eauto. }
+    { ss. eapply Memory.max_full_timemap_closed; eauto. } des.
+
+    exploit Thread.rtc_tau_step_future.
+    { eapply thread_steps_pred_steps. eapply STEPS1. }
+    { ss. eapply Local.cap_wf; eauto. }
+    { ss. eapply Memory.max_full_timemap_closed; eauto. }
+    { ss. eapply Memory.cap_closed; eauto. }
+    i. des. ss.
+
+    destruct th1. exploit no_sc_any_sc_rtc; try apply STEPS1; ss.
+    { i. unfold is_cancel in PR. des_ifs. }
+    i. des. instantiate (1:=sc1) in STEP. clear STEPS1.
+
+    eexists. splits.
+    { eapply STEP. }
+    { ss. ii. clarify.
+      eapply steps_not_cancel_reserves_same in STEPS2; eauto.
+      unguard. des.
+      - eapply NORESERVES; eauto.
+      - rewrite PROMISES in *. erewrite Memory.bot_get in STEPS2. clarify. }
+
+    eapply hold_or_not with (Q := no_acq_read_msgs (caps_loc (Thread.memory th) mem1) /1\ no_sc) in STEPS2. des.
+
+    - destruct e2. ss.
+      exploit no_sc_any_sc_rtc; try eapply HOLD; eauto.
+      { ss. i. des. auto. } i. des.
+      esplits.
+      + eapply pred_step_rtc_mon; try eapply STEP0.
+        i. ss. des. splits; eauto.
+      + ss. unguard. des.
+        * left. ss. inv FAILURE; inv STEP1. inv LOCAL. eauto.
+        * right. esplits; eauto.
+
+    - exploit Thread.rtc_tau_step_future.
+      { eapply thread_steps_pred_steps. eapply STEPS0. }
+      { ss. }
+      { ss. }
+      { ss. } i. des.
+      inv STEP0.
+      exploit Thread.step_future; eauto. i. des.
+
+      assert (PROMS: Local.promise_consistent e3.(Thread.local)).
+      { eapply rtc_tau_step_promise_consistent.
+        - eapply thread_steps_pred_steps. eapply STEPS1.
+        - unguard. des.
+          + inv FAILURE; inv STEP0. inv LOCAL. inv LOCAL0. ss.
+          + ii. rewrite PROMISES in PROMISE.
+            rewrite Memory.bot_get in PROMISE. clarify.
+        - eauto.
+        - eauto.
+        - eauto. }
+
+      assert (NOPROMISE: e2'.(Thread.local).(Local.promises) = Memory.bot).
+      { apply Memory.ext. i. rewrite Memory.bot_get.
+        destruct (Memory.get loc ts (Local.promises (Thread.local e2')))
+          as [[from [val released|]]|] eqn:GET; auto; cycle 1.
+        - exfalso.
+          eapply step_not_cancel_reserves_same in GET; cycle 1.
+          + econs.
+            * econs; eauto.
+            * instantiate (1:=promise_free /1\ (fun e => ~ is_cancel e)). ss.
+          + ss.
+          + des. eapply steps_not_cancel_reserves_same in GET; eauto.
+            des. eapply NORESERVES; eauto.
+        - exfalso.
+          exploit pf_step_rtc_promises_decrease.
+          { eapply STEPS0. }
+          { i. ss. des. auto. }
+          { econs; eauto. } ss. i.
+          exploit pf_step_rtc_promises_decrease.
+          { eapply STEP. }
+          { i. unfold is_cancel in *. des_ifs. }
+          { ss. eauto. }
+          ss. i. inv x2.
+          ss. unfold no_sc, no_acq_read_msgs in BREAKQ. des_ifs; try by (exfalso; eauto).
+
+          + apply not_and_or in BREAKQ. des; clarify.
+            apply imply_to_and in BREAKQ. des. apply NNPP in BREAKQ0.
+            unfold caps_loc in *. des. dup CAPS.
+            eapply caps_unchangable in CAPS; eauto; cycle 1.
+            { inv WF. eauto. }
+            eapply unchangable_rtc_increase in STEP; eauto. ss.
+            eapply unchangable_rtc_increase in STEPS0; eauto. inv STEPS0.
+            inv STEP1; inv STEP0. ss. inv LOCAL.
+            inv LOCAL0. clarify. eapply caps_max_view in CAPS0; eauto; cycle 1.
+            { inv WF. eauto. } des.
+            clarify. eapply PROMS in GET. ss. des_ifs. ss.
+            exploit max_full_timemap_get.
+            * apply MAX.
+            * inv WF. eapply PROMISES. eauto.
+            * i. eapply Time.lt_strorder. eapply TimeFacts.lt_le_lt; eauto.
+              etrans; eauto. eapply TimeMap.join_r.
+          + apply not_and_or in BREAKQ. des; clarify.
+            apply imply_to_and in BREAKQ. des. apply NNPP in BREAKQ0.
+            unfold caps_loc in *. des. dup CAPS.
+            eapply caps_unchangable in CAPS; eauto; cycle 1.
+            { inv WF. eauto. }
+            eapply unchangable_rtc_increase in STEP; eauto. ss.
+            eapply unchangable_rtc_increase in STEPS0; eauto. inv STEPS0.
+            inv STEP1; inv STEP0. ss. inv LOCAL.
+            eapply write_step_promise_consistent in LOCAL2; eauto.
+            inv LOCAL1. clarify. eapply caps_max_view in CAPS0; eauto; cycle 1.
+            { inv WF. eauto. } des.
+            clarify. eapply LOCAL2 in GET. ss. des_ifs. ss.
+            exploit max_full_timemap_get.
+            * apply MAX.
+            * inv WF. eapply PROMISES. eauto.
+            * i. eapply Time.lt_strorder. eapply TimeFacts.lt_le_lt; eauto.
+              etrans; eauto. eapply TimeMap.join_r.
+          + apply not_and_or in BREAKQ. des; clarify. apply NNPP in BREAKQ.
+            inv STEP1; inv STEP0. ss. inv LOCAL. inv LOCAL0. ss.
+            eapply PROMS in GET. ss. des_ifs. ss.
+            hexploit max_full_timemap_get; eauto.
+            * inv WF. eapply Memory.cap_le; eauto.
+            * i. eapply Time.lt_strorder. eapply TimeFacts.lt_le_lt; eauto.
+          + inv STEP1; inv STEP0. ss. inv LOCAL. inv LOCAL0. ss.
+            eapply PROMS in GET. ss. des_ifs. ss.
+            hexploit max_full_timemap_get; eauto.
+            * inv WF. eapply Memory.cap_le; eauto.
+            * i. eapply Time.lt_strorder. eapply TimeFacts.lt_le_lt; eauto.
+      }
+
+      destruct e2'. destruct local. ss.
+      eapply no_sc_any_sc_rtc in STEPS0; ss; cycle 1.
+      { i. des; ss. } des.
+      esplits.
+      * eapply pred_step_rtc_mon; eauto.
+        i. ss. des; auto.
+      * unguard. ss. eauto.
+  Qed.
+
+End PFCONSISTENT.
+
+
+
+Inductive added_memory_imm (tm: TimeMap.t): Memory.t -> Memory.t -> Prop :=
+| added_memory_imm_intro
+    m0 loc to from val m1
+    (TLE: Time.le (tm loc) to)
+    (ADD: Memory.add m0 loc to from (Message.full val None) m1)
+  :
+    added_memory_imm tm m0 m1
 .
 
-Definition mapping_map_lt (f: Loc.t -> Time.t -> Time.t -> Prop): Prop :=
-  forall loc t0 t1 ft0 ft1
-         (MAP0: f loc t0 ft0)
-         (MAP1: f loc t1 ft1),
-    Time.lt t0 t1 -> Time.lt ft0 ft1.
+Definition added_memory (tm: TimeMap.t) := rtc (added_memory_imm tm).
 
-Definition ident_map (loc: Loc.t) := @eq Time.t.
-
-Lemma ident_map_lt
+Lemma added_memory_future tm m0 m1
+      (ADDED: added_memory tm m0 m1)
   :
-    mapping_map_lt ident_map.
+    Memory.future m0 m1.
 Proof.
-  unfold ident_map in *. ii. clarify.
+  ginduction ADDED; auto. etrans; [| apply IHADDED].
+  inv H. econs; eauto. econs; eauto.
+  econs. ss. eapply Time.bot_spec.
 Qed.
 
-Lemma ident_map_le
+Lemma progressable_in_added_rtc
+      lang st lc sc0 sc1 m0 m1 tm
+      (CONSISTENT: Thread.consistent (Thread.mk lang st lc sc0 m0))
+      (FUTURE: Memory.future m0 m1)
   :
-    mapping_map_le ident_map.
+    exists m2 e2,
+      (<<ADDED: rtc (added_memory tm) m1 m2>>) /\
+      (<<STEPS: rtc (Thread.tau_step (lang:=lang))
+                    (Thread.mk _ st lc sc1 m1) e2>>) /\
+      (<<PROMISES: Local.promises (Thread.local e2) = Memory.bot>>).
 Proof.
-  unfold ident_map in *. ii. clarify.
-Qed.
-
-Lemma ident_map_bot
-  :
-    mapping_map_bot ident_map.
-Proof.
-  unfold ident_map in *. ii. clarify.
-Qed.
-
-Lemma ident_map_eq
-  :
-    mapping_map_eq ident_map.
-Proof.
-  unfold ident_map in *. ii. clarify.
-Qed.
-
-Lemma ident_map_total
-      loc to
-  :
-    exists fto,
-      <<MAP: ident_map loc to fto >>.
-Proof.
-  esplits; eauto. refl.
-Qed.
-
-Lemma mapping_map_lt_non_collapsable f
-      (MAPLT: mapping_map_lt f)
-      loc to
-  :
-    non_collapsable f loc to.
-Proof.
-  ii. unfold collapsed in *. des.
-  eapply MAPLT in TLE; eauto. eapply Time.lt_strorder; eauto.
-Qed.
-
-Lemma ident_map_timemap
-      tm
-  :
-    timemap_map ident_map tm tm.
-Proof.
-  ii. refl.
-Qed.
-
-Lemma ident_map_view
-      vw
-  :
-    view_map ident_map vw vw.
-Proof.
-  econs; eapply ident_map_timemap.
-Qed.
-
-Lemma ident_map_message
-      msg
-  :
-    msg_map ident_map msg msg.
-Proof.
-  destruct msg; econs. destruct released; econs.
-  apply ident_map_view.
-Qed.
-
-Lemma ident_map_promises
-      prom
-  :
-    promises_map ident_map prom prom.
-Proof.
-  econs; i.
-  - esplits; eauto.
-    + eapply mapping_map_lt_non_collapsable.
-      eapply ident_map_lt.
-    + refl.
-    + eapply ident_map_message.
-  - esplits; eauto; refl.
-Qed.
-
-Lemma ident_map_local
-      lc
-  :
-    local_map ident_map lc lc.
-Proof.
-  econs; i.
-  - refl.
-  - econs; i; eapply ident_map_view.
-  - eapply ident_map_promises.
-Qed.
-
-Lemma mapping_map_lt_collapsable_unwritable f prom mem
-      (MAPLT: mapping_map_lt f)
-  :
-    collapsable_unwritable f prom mem.
-Proof.
-  ii. exfalso. des.
-  eapply mapping_map_lt_non_collapsable; try eassumption.
-  inv ITV. eapply TimeFacts.lt_le_lt; eauto.
-Qed.
-
-Lemma ident_map_collapsing_latest_memory L prom mem0 mem1 mem2 mem3
-      (MLE: Memory.le prom mem0)
-      (CLOSED: Memory.closed mem0)
-      (LOCS: L = (fun loc => Memory.latest_reserve loc prom mem0))
-      (CAP: Memory.cap prom mem0 mem1)
-      (FORGET0: forget_memory (collapsing_latest_reserves_times L mem0 \2/ collapsing_caps_times L mem0 mem1) mem2 mem1)
-      (FORGET1: forget_memory (latest_other_reserves prom mem0) mem3 mem0)
-  :
-    memory_map ident_map mem2 mem3.
-Proof.
-  econs.
-  - i. dup GET. eapply forget_memory_get in GET0; eauto. des.
-    apply not_or_and in NOT. des.
-    dup GET1. eapply Memory.cap_inv in GET0; eauto. des.
-    + inv FORGET1.
-      erewrite <- COMPLETE in GET0.
-      * right. esplits.
-        { refl. }
-        { eapply ident_map_message. }
-        { refl. }
-        { eauto. }
-      * intros LATEST. inv LATEST.
-        eapply NOT. eexists. econs; eauto. splits; eauto.
-        unfold Memory.latest_reserve. des_ifs.
-    + clarify. left. auto.
-    + clarify. exfalso. eapply NOT0.
-      eexists. econs; eauto. esplits. econs; eauto.
-  - i. dup GET. eapply forget_memory_get in GET0; eauto. des.
-    dup GET1. eapply Memory.cap_le in GET0; eauto; [|refl].
-    inv FORGET0.
-    dup GET0. erewrite <- COMPLETE in GET2.
-    + esplits.
-      * refl.
-      * eauto.
-      * refl.
-    + ii. des.
-      * unfold collapsing_latest_reserves_times, collapsing_latest_reserves, Memory.latest_reserve in H.
-        des. clarify. apply NOT. econs; eauto. des_ifs.
-        eapply MLE in Heq. clarify.
-      * unfold collapsing_caps_times, collapsing_caps, Memory.latest_reserve in H.
-        des. inv CAP0. des. clarify.
-Qed.
-
-Lemma collapsing_latest_memory_concrete_le L prom mem0 mem1 mem2 mem3
-      (MLE: Memory.le prom mem0)
-      (CLOSED: Memory.closed mem0)
-      (LOCS: L = (fun loc => Memory.latest_reserve loc prom mem0))
-      (CAP: Memory.cap prom mem0 mem1)
-      (FORGET0: forget_memory (collapsing_latest_reserves_times L mem0 \2/ collapsing_caps_times L mem0 mem1) mem2 mem1)
-      (FORGET1: forget_memory (latest_other_reserves prom mem0) mem3 mem0)
-  :
-    memory_concrete_le mem2 mem3.
-Proof.
-  ii. dup GET. eapply forget_memory_get in GET0; eauto. des.
-  apply not_or_and in NOT. des.
-  dup GET1. eapply Memory.cap_inv in GET0; eauto. des; clarify.
-  - inv FORGET1.
-    erewrite <- COMPLETE in GET0; eauto.
-    ii. inv H. clarify.
-  - exfalso. eapply NOT0.
-    eexists. econs; eauto. esplits. econs; eauto.
-Qed.
-
-Lemma forget_latest_other_reserves_promises_le prom mem0 mem1
-      (MLE: Memory.le prom mem0)
-      (FORGET: forget_memory (latest_other_reserves prom mem0) mem1 mem0)
-  :
-    Memory.le prom mem1.
-Proof.
-  ii. inv FORGET. erewrite COMPLETE; eauto.
-  ii. inv H. clarify.
-Qed.
-
-Lemma forget_latest_other_reserves_concrete_le prom mem0 mem1
-      (FORGET: forget_memory (latest_other_reserves prom mem0) mem1 mem0)
-  :
-    memory_concrete_le mem0 mem1.
-Proof.
-  ii. inv FORGET. erewrite COMPLETE; eauto.
-  ii. inv H. clarify.
-Qed.
-
-Lemma concrete_le_inhabited mem0 mem1
-      (INHABITED: Memory.inhabited mem0)
-      (MLE: memory_concrete_le mem0 mem1)
-  :
-    Memory.inhabited mem1.
-Proof.
-  ii. eapply MLE; eauto.
-Qed.
-
-Lemma forget_latest_other_reserves_closed prom mem0 mem1
-      (CLOSED: Memory.closed mem0)
-      (MLE: Memory.le prom mem0)
-      (FORGET: forget_memory (latest_other_reserves prom mem0) mem1 mem0)
-  :
-    Memory.closed mem1.
-Proof.
-  inv CLOSED. econs; eauto.
-  - i. dup MSG. eapply forget_memory_get in MSG; eauto. des.
-    dup GET. eapply CLOSED0 in GET0. des. splits; auto.
-    eapply memory_concrete_le_closed_msg; eauto.
-    eapply forget_latest_other_reserves_concrete_le; eauto.
-  - eapply concrete_le_inhabited; eauto.
-    eapply forget_latest_other_reserves_concrete_le; eauto.
-Qed.
-
-Definition my_max_timemap (prom mem: Memory.t) (tm: TimeMap.t): Prop :=
-  forall loc,
-    ((<<MAX: Memory.max_full_ts mem loc (tm loc)>>) /\
-     (<<LATEST: Memory.latest_reserve loc prom mem>>)) \/
-    ((<<MAX: Memory.max_ts loc mem = (tm loc)>>) /\
-     (<<LATEST: ~ Memory.latest_reserve loc prom mem>>)).
-
-Lemma my_max_timemap_exists prom mem
-      (INHABITED: Memory.inhabited mem)
-  :
-    exists tm, <<MYMAX: my_max_timemap prom mem tm>>.
-Proof.
-  exploit (choice
-             (fun loc to =>
-                ((<<MAX: Memory.max_full_ts mem loc to>>) /\
-                 (<<LATEST: Memory.latest_reserve loc prom mem>>)) \/
-                ((<<MAX: Memory.max_ts loc mem = to>>) /\
-                 (<<LATEST: ~ Memory.latest_reserve loc prom mem>>)))).
-  - i. destruct (classic (Memory.latest_reserve x prom mem)).
-    + exploit Memory.max_full_ts_exists; eauto.
-      i. des. esplits. left. split; eauto.
-    + esplits. right. split; eauto.
-  - i. des. exists f. esplits; eauto.
-Qed.
-
-Lemma my_max_timemap_inj prom mem tm0 tm1
-      (MYMAX0: my_max_timemap prom mem tm0)
-      (MYMAX1: my_max_timemap prom mem tm1)
-  :
-    tm0 = tm1.
-Proof.
-  extensionality loc.
-  specialize (MYMAX0 loc). specialize (MYMAX1 loc). des; clarify.
-  - eapply Memory.max_full_ts_inj; eauto.
-  - rewrite <- MAX0. auto.
-Qed.
-
-Lemma memory_cap_covered prom mem0 mem1
-      (CAP: Memory.cap prom mem0 mem1)
-      (INHABITED: Memory.inhabited mem0)
-      loc to
-      (TS0: Time.lt Time.bot to)
-      (TS1: Time.le to (Memory.max_ts loc mem0))
-  :
-    covered loc to mem1.
-Proof.
-  inv CAP.
-  set (@cell_elements_least
-         (mem0 loc)
-         (fun to' => Time.le to to')). des; cycle 1.
-  { exfalso. exploit Memory.max_ts_spec.
-    - eapply INHABITED.
-    - i. des. exploit EMPTY; eauto. }
-  set (@cell_elements_greatest
-         (mem0 loc)
-         (fun to' => Time.lt to' to)). des; cycle 1.
-  { exfalso. exploit EMPTY.
-    - eapply INHABITED.
-    - eauto.
-    - ss. }
-  destruct (Time.le_lt_dec to from).
-  - exploit MIDDLE.
-    + econs.
-      * eapply GET0.
-      * eapply GET.
-      * eapply TimeFacts.lt_le_lt; eauto.
-      * i. destruct (Memory.get loc ts mem0) eqn:GET1; auto.
-        exfalso. destruct p.
-        destruct (Time.le_lt_dec to ts).
-        { exploit LEAST; eauto. i.
-          eapply Time.lt_strorder. eapply TimeFacts.le_lt_lt.
-          { eapply x. }
-          eapply TimeFacts.le_lt_lt.
-          { eapply TS3. }
-          { eapply memory_get_ts_strong in GET. des; clarify; ss.
-            exfalso. eapply Time.lt_strorder. eapply TimeFacts.le_lt_lt.
-            - eapply l.
-            - eauto. } }
-        { exploit GREATEST; eauto. i.
-          eapply Time.lt_strorder. eapply TimeFacts.le_lt_lt.
-          { eapply x. }
-          { eauto. } }
-    + eapply TimeFacts.lt_le_lt; eauto.
-    + i. econs; eauto. econs; eauto.
-  - econs.
-    + eapply Memory.cap_le; try apply GET; eauto. refl.
-    + econs; eauto.
-Qed.
-
-Definition later_times (tm: TimeMap.t) (loc: Loc.t) (to: Time.t): Prop :=
-  Time.lt (tm loc) to.
-
-Lemma forget_covered L mem0 mem1
-      (FORGET: forget_memory L mem1 mem0)
-      loc ts
-      (COVERED: covered loc ts mem0)
-      (KEEP: forall to from msg (SAT: L loc to)
-                    (GET: Memory.get loc to mem0 = Some (from, msg)),
-          ~ Interval.mem (from, to) ts)
-  :
-    covered loc ts mem1.
-Proof.
-  inv COVERED. inv FORGET.
-  erewrite <- COMPLETE in GET.
-  - econs; eauto.
-  - ii. eapply KEEP in H; eauto.
-Qed.
-
-Lemma memory_reserve_wf_mon prom0 prom1 mem
-      (RESERVEWF: Memory.reserve_wf prom1 mem)
-      (MLE: Memory.le prom0 prom1)
-  :
-    Memory.reserve_wf prom0 mem.
-Proof.
-  ii. eauto.
-Qed.
-
-Lemma ident_map_mappable_any_event e
-  :
-    mappable_evt ident_map e.
-Proof.
-  destruct e; ss; split; eapply ident_map_total.
-Qed.
-  
-Lemma collapsing_last_reserves_promise_or_later
-      L prom mem0 mem1 mem2 max
-      (LOC: L = (fun loc => Memory.latest_reserve loc prom mem0))
-      (MLE: Memory.le prom mem0)
-      (RESERVEWF: memory_reserve_wf mem0)
-      (CLOSED: Memory.closed mem0)
-      (CAP: Memory.cap prom mem0 mem1)
-      (MAX: my_max_timemap prom mem0 max)
-      (FORGET: forget_memory (collapsing_latest_reserves_times L mem0 \2/ collapsing_caps_times L mem0 mem1) mem2 mem1)
-      loc to
-      (UNWRITABLE: ~ unwritable mem2 prom loc to)
-  :
-    <<COVERED: covered loc to prom>> \/ <<LATER: later_times max loc to>> \/ <<BOT: to = Time.bot>>.
-Proof.
-  clarify.
-  assert (RESERVEWF0: Memory.reserve_wf prom mem0).
-  { eapply memory_reserve_wf_mon; eauto. }
-  assert (INHABITED: Memory.inhabited mem0).
-  { inv CLOSED. eauto. }
-  assert (MLE0: Memory.le prom mem2).
-  { eapply collapsing_caps_forget_prom_le; eauto.
-    ii. clarify. unfold Memory.latest_reserve in SAT. des_ifs. }
-  erewrite unwritable_eq in UNWRITABLE; eauto.
-  eapply not_and_or in UNWRITABLE. des.
-  - destruct (Time.le_lt_dec to Time.bot).
-    { right. right. destruct l; auto. exfalso.
-      eapply Time.lt_strorder. eapply TimeFacts.lt_le_lt; eauto.
-      eapply Time.bot_spec. }
-    right. left.
-    destruct (Time.le_lt_dec to (max loc)); auto. exfalso.
-    eapply UNWRITABLE. red.
-    eapply forget_covered; eauto.
-    + eapply memory_cap_covered; eauto.
-      etrans; eauto. specialize (MAX loc). des; clarify.
-      { eapply max_full_ts_le_max_ts; eauto. }
-      { rewrite <- MAX0. refl. }
-    + ii. inv H. ss. des.
-      * unfold collapsing_latest_reserves_times, collapsing_latest_reserves in SAT.
-        des. clarify. specialize (MAX loc). des; clarify.
-        dup RESERVE. eapply Memory.cap_le in RESERVE0; eauto; [|refl]. clarify.
-        eapply max_ts_reserve_from_full_ts in RESERVE; eauto.
-        exploit Memory.max_full_ts_inj.
-        { eapply RESERVE. }
-        { eapply MAX0. }
-        i. clarify. eapply Time.lt_strorder.
-        eapply TimeFacts.lt_le_lt; eauto.
-      * unfold collapsing_caps_times, collapsing_caps, caps in SAT. des. clarify.
-        exploit Memory.cap_inv; eauto. i. des; clarify.
-        eapply Time.lt_strorder. eapply TimeFacts.lt_le_lt.
-        { eapply FROM. }
-        etrans.
-        { eapply l0. }
-        { specialize (MAX loc). des; clarify.
-          eapply max_full_ts_le_max_ts; eauto. }
-  - apply NNPP in UNWRITABLE. auto.
-Qed.
-
-Lemma write_not_in_write_in L0 L1
-      (LOCS: forall loc to (NSAT: ~ L0 loc to),
-          <<SAT: L1 loc to>> \/ <<BOT: to = Time.bot>>)
-  :
-    write_not_in L0 <1= write_in L1.
-Proof.
-  i. destruct x0; ss.
-  - i. dup IN. eapply PR in IN. eapply LOCS in IN. des; auto.
-    clarify. inv IN0. ss. exfalso.
-    eapply Time.lt_strorder. eapply TimeFacts.lt_le_lt.
-    + eapply FROM.
-    + eapply Time.bot_spec.
-  - i. dup IN. eapply PR in IN. eapply LOCS in IN. des; auto.
-    clarify. inv IN0. ss. exfalso.
-    eapply Time.lt_strorder. eapply TimeFacts.lt_le_lt.
-    + eapply FROM.
-    + eapply Time.bot_spec.
-Qed.
-
-Definition pf_consistent_drf lang (e0:Thread.t lang): Prop :=
-  let L := (fun loc => Memory.latest_reserve loc e0.(Thread.local).(Local.promises) e0.(Thread.memory)) in
-  forall mem1 max sc
-         (FORGET: forget_memory (latest_other_reserves e0.(Thread.local).(Local.promises) e0.(Thread.memory)) mem1 e0.(Thread.memory))
-         (MAX: my_max_timemap e0.(Thread.local).(Local.promises) e0.(Thread.memory) max),
-  exists e1,
-    (<<STEPS0: rtc (tau (@pred_step ((promise_free /1\ no_acq_update_msgs ((fun loc to => L loc) /2\ Memory.max_full_ts e0.(Thread.memory))) /1\ no_sc /1\ write_in (later_times max \2/ fun loc to => covered loc to e0.(Thread.local).(Local.promises))) lang)) (Thread.mk _ e0.(Thread.state) e0.(Thread.local) sc mem1) e1>>) /\
-    (__guard__((<<FAILURE: Local.failure_step e1.(Thread.local)>>) \/
-               (<<PROMISES: e1.(Thread.local).(Local.promises) = Memory.bot>>))).
-
-Lemma pf_consistent_pf_consistent_drf lang (th: Thread.t lang)
-      (WF: Local.wf th.(Thread.local) th.(Thread.memory))
-      (MEM: Memory.closed th.(Thread.memory))
-      (CONSISTENT: pf_consistent th)
-      (RESERVEWF: memory_reserve_wf (Thread.memory th))
-  :
-    pf_consistent_drf th.
-Proof.
-  eapply pf_consistent_pf_consistent_strong in CONSISTENT; eauto.
-  eapply pf_consistent_pf_consistent_drf' in CONSISTENT; eauto.
-  eapply pf_consistent_pf_consistent_drf'' in CONSISTENT; eauto.
-  
-  set (L:=fun loc : Loc.t =>
-            Memory.latest_reserve loc (Local.promises (Thread.local th)) (Thread.memory th)).
-  exploit Memory.cap_exists; eauto. i. des.
-  exploit forget_exists; eauto. i. des.
-  ii. exploit CONSISTENT; eauto. i. des.
-  assert (MLE0: Memory.le (Local.promises (Thread.local th)) (Thread.memory th)).
-  { inv WF. auto. }
-  assert (COLLAPSABLE: collapsable_cap L (Local.promises (Thread.local th)) (Thread.memory th)).
-  { ii. clarify. unfold L, Memory.latest_reserve in SAT.
-    rewrite GET in SAT. clarify. }
-  assert (MEMORY: memory_map ident_map mem_src mem1).
-  { eapply ident_map_collapsing_latest_memory; cycle 3; eauto. }
-  assert (MLE1: memory_concrete_le mem_src mem1).
-  { eapply collapsing_latest_memory_concrete_le; cycle 3; eauto. }
-  assert (CONCRETELE: memory_concrete_le th.(Thread.memory) mem_src).
-  { eapply collapsing_caps_forget_le; eauto. }
-  assert (LCWFTGT: Local.wf th.(Thread.local) mem_src).
-  { eapply memory_concrete_le_local_wf; eauto. inv WF.
-    eapply collapsing_caps_forget_prom_le; eauto. } 
-  assert (LCWFSRC: Local.wf th.(Thread.local) mem1).
-  { eapply memory_concrete_le_local_wf; eauto. inv WF.
-    eapply forget_latest_other_reserves_promises_le; eauto. }
-  assert (CLOSEDSRC: Memory.closed mem1).
-  { eapply forget_latest_other_reserves_closed; cycle 1; eauto. }
-  assert (CLOSEDTGT: Memory.closed mem_src).
-  { eapply collapsing_caps_forget_closed; cycle 1; eauto. }
-  eapply steps_write_not_in in STEPS0; ss; cycle 1.
-  { eauto. inv LCWFTGT. auto. }
-  eapply steps_wf_event in STEPS0; ss; cycle 1.
-  { inv CLOSEDTGT. auto. }
-  
-  destruct e1.
-  hexploit (@steps_map ident_map); try apply STEPS0; try apply MEMORY; eauto.
-  { eapply ident_map_le. }
-  { eapply ident_map_bot. }
-  { eapply ident_map_eq. }
-  { ss. i. eapply ident_map_mappable_any_event. }
-  { eapply Memory.closed_timemap_bot; eauto. inv CLOSEDSRC. auto. }
-  { eapply Memory.closed_timemap_bot; eauto. inv CLOSEDTGT. auto. }
-  { eapply ident_map_local; eauto. }
-  { eapply mapping_map_lt_collapsable_unwritable. eapply ident_map_lt. }
-  { eapply ident_map_timemap. }
-  { refl. }
-  { instantiate (1:=(promise_free /1\ no_acq_update_msgs ((fun loc to => L loc) /2\ Memory.max_full_ts th.(Thread.memory))) /1\ no_sc /1\ write_in (later_times max \2/ fun loc to => covered loc to th.(Thread.local).(Local.promises))).
-    ii. ss. des. splits.
-    - inv REL; ss. inv KIND; ss. inv MSG0; ss. inv MSG; ss. inv MAP0; ss.
-    - inv REL; ss. inv FROM. ss.
-    - inv REL; ss.
-    - eapply write_not_in_write_in in SAT1.
-      + instantiate (1:=later_times max \2/ fun loc to => covered loc to th.(Thread.local).(Local.promises)) in SAT1.
-        inv REL; ss.
-        * inv FROM. inv TO. eauto.
-        * inv FROM. inv TO. eauto.
-      + i. eapply collapsing_last_reserves_promise_or_later in NSAT; ss; eauto.
-        des; auto. }
-  i. des.
-  eapply no_sc_any_sc_rtc in STEP; ss; cycle 1.
-  { i. destruct x1; ss; des; auto. } des.
-  esplits; eauto.
-  unguard. des; ss.
-  - left. econs. inv FAILURE. inv LOCAL.
-    eapply promise_consistent_mon.
-    { eapply promise_consistent_map; eauto.
-      - eapply ident_map_le.
-      - eapply ident_map_eq. }
-    { ss. }
-    { ss. }
-  - right. inv LOCAL. rewrite PROMISES in *.
-    eapply bot_promises_map; eauto.
-Qed.
-
-
-Definition times_in_memory (mem: Memory.t) (L: Loc.t -> list Time.t): Prop :=
-  forall loc t,
-    (<<SAT: List.In t (L loc)>>) <->
-    (<<INMEMORY:
-       (exists from msg, (<<GET: Memory.get loc t mem = Some (from, msg)>>)) \/
-       (exists to msg, (<<GET: Memory.get loc to mem = Some (t, msg)>>))>>).
-
-Lemma times_in_memory_exists mem
-  :
-    exists l, times_in_memory mem l.
-Proof.
-  hexploit (choice
-              (fun loc tl =>
-                 forall t,
-                   (<<SAT: List.In t tl>>) <->
-                   (<<INMEMORY:
-                      (exists from msg, (<<GET: Memory.get loc t mem = Some (from, msg)>>)) \/
-                      (exists to msg, (<<GET: Memory.get loc to mem = Some (t, msg)>>))>>))); auto.
-  intros loc.
-  hexploit (wf_cell_msgs_exists (mem loc)). i. des.
-  exists ((List.map (fun ftm =>
-                       match ftm with
-                       | (from, _, _) => from
-                       end) l)
-            ++
-            (List.map (fun ftm =>
-                         match ftm with
-                         | (_, to, _) => to
-                         end) l)).
-  i. split; i.
-  - red in H. eapply List.in_app_or in H. des.
-    + eapply List.in_map_iff in H. des.
-      destruct x as [[from to] msg]. clarify.
-      eapply COMPLETE in H0. right. eauto.
-    + eapply List.in_map_iff in H. des.
-      destruct x as [[from to] msg]. clarify.
-      eapply COMPLETE in H0. left. eauto.
-  - eapply List.in_or_app.  des.
-    + right. eapply COMPLETE in GET.
-      eapply List.in_map_iff. esplits; eauto. ss.
-    + left. eapply COMPLETE in GET.
-      eapply List.in_map_iff. esplits; eauto. ss.
-Qed.
-
-
-
-(* Inductive shifted_map mlast mcert *)
-(*           (updates: Loc.t -> Prop) *)
-(*           (sky gap: TimeMap.t) *)
-(*           (f: Loc.t -> Time.t -> Time.t): Prop := *)
-(* | shifted_map_intro *)
-(*     (PRSV: map_preserving (times_in_memory mcert) f) *)
-(*     (SAME: forall l t (TLE: Time.le t (Memory.max_ts l mlast)), *)
-(*         f l t = t) *)
-(*     (INGAP: forall l t (TLT: Time.lt (Memory.max_ts l mcert) t), *)
-(*         Time.lt (f l t) (gap l)) *)
-(*     (AFTERSKY: forall l t (TLT: Time.lt (Memory.max_ts l mcert) t), *)
-(*         Time.lt (sky l) (f l t)) *)
-(* . *)
-
-(* Lemma shifted_map_exists mlast mcert updates *)
-(*       (MLE: Memory.le mlast mcert) *)
-(*       (sky gap: TimeMap.t) *)
-(*       (SKY: forall l, Time.lt (Memory.max_ts l mlast) (sky l)) *)
-(*       (GAP: forall l, Time.lt (Memory.max_ts l mlast) (gap l)) *)
-(*   : *)
-(*     exists f, (<<SHIFTED: shifted_map mlast mcert updates sky gap f>>). *)
-(* Proof. *)
-(*   (* may be very hard... *) *)
-(* Admitted. *)
-
-(* Lemma shifted_map_preserving_last_mem  mlast mcert updates sky gap f *)
-(*       (CLOSED: Memory.closed mlast) *)
-(*       (SHIFTED: shifted_map mlast mcert updates sky gap f) *)
-(*   : *)
-(*     memory_map f mlast mlast. *)
-(* Proof. *)
-(*   inv SHIFTED. inv PRSV. econs; i. *)
-(*   - exploit Memory.max_ts_spec; eauto. i. des. *)
-(*     repeat erewrite SAME; eauto. *)
-(*     + rewrite GET. unfold msg_map. des_ifs. repeat f_equal. *)
-(*       inv CLOSED. exploit CLOSED0; try apply GET; eauto. i. des. *)
-(*       inv MSG_CLOSED. inv CLOSED; ss. f_equal. *)
-(*       destruct view. inv CLOSED1. unfold view_map, timemap_map. ss. f_equal. *)
-(*       * extensionality l. erewrite SAME; auto. *)
-(*         specialize (PLN l). des. *)
-(*         exploit Memory.max_ts_spec; eauto. i. des. auto. *)
-(*       * extensionality l. erewrite SAME; auto. *)
-(*         specialize (RLX l). des. *)
-(*         exploit Memory.max_ts_spec; eauto. i. des. auto. *)
-(*     + exploit Memory.get_ts; try apply GET; eauto. i. des. *)
-(*       * clarify. *)
-(*       * left. eapply TimeFacts.lt_le_lt; eauto. *)
-(*   - destruct msg_src as [from msg]. exploit Memory.max_ts_spec; eauto. i. des. *)
-(*     esplits. *)
-(*     + erewrite SAME; eauto. *)
-(*     + eauto. *)
-(* Qed. *)
-
-
-
-
-
-
-(* Inductive add_cap (caps: Loc.t -> option (Time.t * Time.t * Message.t)): Memory.t -> Memory.t -> Prop := *)
-(* | add_cap_refl mem0 *)
-(*   : *)
-(*     add_cap caps mem0 mem0 *)
-(* | add_cap_add *)
-(*     loc from to msg mem0 mem1 *)
-(*     (CAP: caps loc = Some (from, to, msg)) *)
-(*     (ADD: Memory.add mem0 loc from to msg mem1) *)
-(*   : *)
-(*     add_cap caps mem0 mem1 *)
-(* . *)
-(* Hint Constructors add_cap. *)
-
-
-(* Lemma diff_after_promise_write caps prom0 mem_src0 mem_tgt0 *)
-(*       loc from to val released kind prom1 mem_tgt1 *)
-(*       (DIFF: diff_after_promises caps prom0 mem_src0 mem_tgt0) *)
-(*       (CAPSWF: forall loc from to msg (CAP: caps loc = Some (from, to, msg)), *)
-(*           Time.lt from to) *)
-(*       (MLE: Memory.le prom0 mem_src0) *)
-(*       (WRITE: Memory.write prom0 mem_tgt0 loc from to val released prom1 mem_tgt1 kind) *)
-(*   : *)
-(*     exists mem_src1' mem_src1, *)
-(*       (<<WRITE: Memory.write prom0 mem_src0 loc from to val released prom1 mem_src1' kind>>) /\ *)
-(*       (<<ADD: add_cap caps mem_src1' mem_src1>>) /\ *)
-(*       (<<DIFF: diff_after_promises caps prom1 mem_src1 mem_tgt1>>). *)
-(* Proof. *)
-(*   dup DIFF. inv DIFF. inv WRITE; ss. *)
-(*   generalize (unchangable_promise PROMISE). intros UNCH. *)
-(*   inv PROMISE; ss. *)
-(*   - exploit Memory.add_exists_le. *)
-(*     { eapply MLE0. } *)
-(*     { eapply MEM. } *)
-(*     intros [mem_src' ADD]. exists mem_src', mem_src'. splits; auto. *)
-(*     + econs; eauto. econs; eauto. i. clarify. *)
-(*     + assert (PROM: prom1 = prom0). *)
-(*       { eapply MemoryFacts.MemoryFacts.add_remove_eq; eauto. } clarify. *)
-(*       econs. *)
-(*       * eapply memory_op_le; eauto. *)
-(*       * i. erewrite Memory.add_o in GET; eauto. *)
-(*         erewrite Memory.add_o in NONE; eauto. des_ifs. guardH o. *)
-(*         exploit DIFF1; eauto. *)
-(*       * i. exploit UNCH. *)
-(*         { eapply diff_after_promise_unchangable; eauto. } i. inv x. *)
-(*         eapply CAPS in CAP. des. splits; eauto. *)
-(*         { i. erewrite Memory.add_o in NONE; eauto. des_ifs. guardH o. *)
-(*           eapply SRCGET in NONE. eauto. } *)
-(*         { i. eapply PROM in PROM0. des. split; auto. *)
-(*           erewrite Memory.add_o; eauto. des_ifs. ss. des; clarify. *)
-(*           eapply Memory.add_get0 in MEM. des. clarify. } *)
-
-(*   - exploit Memory.split_exists_le. *)
-(*     { eapply MLE. } *)
-(*     { eapply PROMISES. } *)
-(*     intros [mem_src' SPLIT]. exists mem_src', mem_src'. splits; auto. *)
-(*     + econs; eauto. *)
-(*     + econs. *)
-(*       * eapply memory_op_le; eauto. *)
-(*       * i. erewrite Memory.split_o in GET; eauto. *)
-(*         erewrite Memory.split_o in NONE; eauto. des_ifs. guardH o. guardH o0. *)
-(*         exploit DIFF1; eauto. *)
-(*       * i. exploit UNCH. *)
-(*         { eapply diff_after_promise_unchangable; eauto. } i. inv x. *)
-(*         eapply CAPS in CAP. des. splits; eauto. *)
-(*         { erewrite Memory.remove_o; eauto. des_ifs. } *)
-(*         { i. erewrite Memory.split_o in NONE; eauto. des_ifs. *)
-(*           guardH o. guardH o0. eapply SRCGET in NONE. des. *)
-(*           dup PROM0. eapply Memory.split_get1 in PROM0; eauto. des. *)
-(*           eapply Memory.remove_get1 in GET2; eauto. ss. des; clarify. *)
-(*           - eapply Memory.split_get0 in PROMISES. des. clarify. *)
-(*           - esplits; eauto. } *)
-(*         { dup PROMISES. eapply Memory.split_get0 in PROMISES; eauto. des. *)
-(*           i. erewrite Memory.remove_o in PROM0; eauto. des_ifs. guardH o. *)
-(*           erewrite Memory.split_o in PROM0; eauto. des_ifs; ss; clarify. *)
-(*           - unguard. des; clarify. *)
-(*           - guardH o0. des; clarify. *)
-(*             eapply PROM in GET1. des. split; auto. *)
-(*             erewrite Memory.split_o; eauto. des_ifs. *)
-(*             + ss. des; clarify. *)
-(*             + guardH o1. ss. des; clarify. *)
-(*           - guardH o0. guardH o1. dup PROM0. eapply PROM in PROM0. *)
-(*             des. split; auto. *)
-(*             erewrite Memory.split_o; eauto. des_ifs. *)
-(*             + ss. unguard. des; clarify. *)
-(*             + ss. unguard. des; clarify. } *)
-
-(*   - exploit Memory.lower_exists_le. *)
-(*     { eapply MLE. } *)
-(*     { eapply PROMISES. } *)
-(*     intros [mem_src' LOWER]. *)
-
-(*     destruct (classic ((forall to' from' msg *)
-(*                                (GET: Memory.get loc to' prom1 = Some (from', msg)), *)
-(*                            msg = Message.reserve) /\ *)
-(*                        exists p, (<<CAP: caps loc = Some p>>))). *)
-(*     { des. destruct p as [[from1 to1] msg1]. *)
-(*       dup CAP. eapply CAPS in CAP. des. *)
-(*       exploit UNCH. *)
-(*       { eapply diff_after_promise_unchangable; eauto. } i. inv x. *)
-(*       hexploit (@Memory.add_exists mem_src' loc from1 to1 msg1); eauto. *)
-(*       { i. dup GET2. eapply memory_op_le in GET2; eauto. *)
-(*         exploit Memory.get_disjoint. *)
-(*         - eapply GET. *)
-(*         - eapply GET2. *)
-(*         - i. des; clarify. exfalso. *)
-(*           eapply Memory.lower_get0 in PROMISES. des. *)
-(*           eapply PROM in GET1. des. *)
-(*           erewrite Memory.lower_o in GET0; eauto. des_ifs; ss; des; clarify. } *)
-(*       { eapply Cell.get_opt_wf; eauto. } *)
-(*       intros [mem_src'' ADD]. exists mem_src', mem_src''. *)
-(*       splits; eauto. econs. *)
-(*       - hexploit memory_op_le; eauto. intros MLE1. *)
-(*         ii. erewrite Memory.add_o in LHS; eauto. des_ifs; eauto. *)
-(*         ss. des; clarify. *)
-(*       - i. erewrite Memory.add_o in NONE; eauto. des_ifs. guardH o. *)
-(*         erewrite Memory.lower_o in GET0; eauto. *)
-(*         erewrite Memory.lower_o in NONE; eauto. des_ifs. eapply DIFF1; eauto. *)
-(*       - i. exploit UNCH. *)
-(*         { eapply diff_after_promise_unchangable; eauto. } i. inv x. *)
-(*         dup CAP. eapply CAPS in CAP. des. splits; eauto. *)
-(*         + erewrite Memory.remove_o; eauto. des_ifs. *)
-(*         + i. erewrite Memory.add_o in NONE; eauto. des_ifs. guardH o. *)
-(*           erewrite Memory.lower_o in NONE; eauto. des_ifs. guardH o0. *)
-(*           eapply SRCGET0 in NONE. des. *)
-(*           eapply Memory.lower_get1 in PROM1; eauto. des. inv MSG_LE. *)
-(*           eapply Memory.remove_get1 in GET2; eauto. des; clarify; eauto. *)
-(*           ss. unguard. des; clarify. *)
-(*         + i. dup PROM1. erewrite Memory.remove_o in PROM2; eauto. des_ifs. *)
-(*           guardH o. erewrite Memory.lower_o in PROM2; eauto. des_ifs. *)
-(*           * ss. unguard. des; clarify. *)
-(*           * guardH o0. ss. eapply PROM0 in PROM2. des. split; auto. *)
-(*             erewrite Memory.add_o; eauto. des_ifs. *)
-(*             { ss. des; clarify. eapply H in PROM1. clarify. } *)
-(*             { erewrite Memory.lower_o; eauto. des_ifs. *)
-(*               unguard. ss. des;clarify. } *)
-(*     } *)
-(*     { exists mem_src', mem_src'. splits; auto. *)
-(*       + econs; eauto. *)
-(*       + econs. *)
-(*         * eapply memory_op_le; eauto. *)
-(*         * i. erewrite Memory.lower_o in GET; eauto. *)
-(*           erewrite Memory.lower_o in NONE; eauto. des_ifs. guardH o. *)
-(*           exploit DIFF1; eauto. *)
-(*         * i. exploit UNCH. *)
-(*           { eapply diff_after_promise_unchangable; eauto. } i. inv x. *)
-(*           dup CAP. eapply CAPS in CAP. des. splits; eauto. *)
-(*           { erewrite Memory.remove_o; eauto. des_ifs. } *)
-(*           { i. erewrite Memory.lower_o in NONE; eauto. des_ifs. *)
-(*             guardH o. eapply SRCGET in NONE. des. *)
-(*             dup PROM0. eapply Memory.lower_get1 in PROM0; eauto. des. *)
-(*             eapply Memory.remove_get1 in GET2; eauto. ss. des; clarify. *)
-(*             - apply not_and_or in H. des. *)
-(*               + eapply not_all_ex_not in H. destruct H as [from1 H]. *)
-(*                 eapply not_all_ex_not in H. destruct H as [to1 H]. *)
-(*                 eapply not_all_ex_not in H. destruct H as [msg1 H]. *)
-(*                 eapply imply_to_and in H. destruct H as [GET0 CONCRETE]. *)
-(*                 destruct msg1; clarify. esplits; eauto. *)
-(*               + exfalso. eapply H. esplits; eauto. *)
-(*             - inv MSG_LE. esplits; eauto. } *)
-(*           { dup PROMISES. eapply Memory.lower_get0 in PROMISES; eauto. des. *)
-(*             i. erewrite Memory.remove_o in PROM0; eauto. des_ifs. guardH o. *)
-(*             erewrite Memory.lower_o in PROM0; eauto. des_ifs; ss; clarify. *)
-(*             - unguard. des; clarify. *)
-(*             - guardH o0. eapply PROM in PROM0. des. split; auto. *)
-(*               erewrite Memory.lower_o; eauto. des_ifs. *)
-(*               ss. des; clarify. } *)
-(*     } *)
-(* Qed. *)
-
-(* Lemma diff_after_promises_step caps P lang *)
-(*       th_src th_tgt th_tgt' st st' v v' prom prom' sc sc' *)
-(*       mem_src mem_tgt mem_tgt' e *)
-(*       (CAPSWF: forall loc from to msg (CAP: caps loc = Some (from, to, msg)), *)
-(*           Time.lt from to) *)
-(*       (MLE: Memory.le prom mem_src) *)
-(*       (STEP: (@pred_step P lang) e th_tgt th_tgt') *)
-(*       (PROMISEFREE: P <1= promise_free) *)
-(*       (TH_SRC: th_src = Thread.mk lang st (Local.mk v prom) sc mem_src) *)
-(*       (TH_TGT0: th_tgt = Thread.mk lang st (Local.mk v prom) sc mem_tgt) *)
-(*       (TH_TGT1: th_tgt' = Thread.mk lang st' (Local.mk v' prom') sc' mem_tgt') *)
-(*       (DIFF: diff_after_promises caps prom mem_src mem_tgt) *)
-(*       (CONSISTENT: Local.promise_consistent (Local.mk v' prom')) *)
-(*   : *)
-(*     exists mem_src' mem_src'', *)
-(*       (<<STEP: (@pred_step P lang) *)
-(*                  e th_src *)
-(*                  (Thread.mk lang st' (Local.mk v' prom') sc' mem_src')>>) /\ *)
-(*       (<<ADD: add_cap caps mem_src' mem_src''>>) /\ *)
-(*       (<<DIFF: diff_after_promises caps prom' mem_src'' mem_tgt'>>) *)
-(* . *)
-(* Proof. *)
-(*   inv STEP. dup SAT. eapply PROMISEFREE in SAT. inv STEP0. inv STEP. *)
-(*   - inv STEP0. inv LOCAL. ss. clarify. *)
-(*     exploit diff_after_promise_promise; eauto. *)
-(*     i. des. exists mem_src1, mem_src1. splits; eauto. *)
-(*     econs; eauto. econs; eauto. econs 1; eauto. *)
-(*     econs; eauto. econs; eauto. *)
-(*     unfold Message.is_released_none, Memory.op_kind_is_cancel, andb, orb in *. *)
-(*     des_ifs. *)
-(*     + econs. econs. *)
-(*     + inv PROMISE. econs. *)
-(*   - inv STEP0. inv LOCAL; ss. *)
-(*     + exists mem_src, mem_src. splits; eauto. *)
-(*       econs; eauto. econs; eauto. *)
-(*     + dup LOCAL0. inv LOCAL0. ss. clarify. *)
-(*       assert (GETSRC: Memory.get loc ts mem_src = Some (from, Message.full val released)). *)
-(*       { inv DIFF. destruct (Memory.get loc ts mem_src) eqn: GET0. *)
-(*         - destruct p. eapply MLE0 in GET0. clarify. *)
-(*         - exploit DIFF0; eauto. intros CAP. *)
-(*           eapply CAPS in CAP. des. eapply SRCGET in GET0. des. *)
-(*           dup PROM0. eapply PROM in PROM0. des. *)
-(*           exploit promise_consistent_promise_read; eauto. *)
-(*           i. exfalso. eapply Time.lt_strorder. etrans; eauto. } *)
-(*       exists mem_src, mem_src. splits; eauto. *)
-(*       econs; eauto. econs; eauto. *)
-(*     + inv LOCAL0. ss. clarify. *)
-(*       exploit diff_after_promise_write; eauto. i. des. *)
-(*       exists mem_src1', mem_src1. splits; eauto. *)
-(*       econs; eauto. econs; eauto. *)
-(*     + eapply write_step_promise_consistent in CONSISTENT; eauto. *)
-(*       dup LOCAL1. inv LOCAL1. inv LOCAL2. ss. clarify. *)
-(*       assert (GETSRC: Memory.get loc tsr mem_src = Some (from, Message.full valr releasedr)). *)
-(*       { inv DIFF. destruct (Memory.get loc tsr mem_src) eqn: GET0. *)
-(*         - destruct p. eapply MLE0 in GET0. clarify. *)
-(*         - exploit DIFF0; eauto. intros CAP. *)
-(*           eapply CAPS in CAP. des. eapply SRCGET in GET0. des. *)
-(*           dup PROM0. eapply PROM in PROM0. des. *)
-(*           exploit promise_consistent_promise_read; eauto. *)
-(*           i. exfalso. eapply Time.lt_strorder. etrans; eauto. } *)
-(*       exploit diff_after_promise_write; eauto. i. des. *)
-(*       exists mem_src1', mem_src1. splits; eauto. *)
-(*       econs; eauto. econs; eauto. econs 2; eauto. *)
-(*     + inv LOCAL0. ss. clarify. *)
-(*       exists mem_src, mem_src. splits; eauto. *)
-(*       econs; eauto. econs; eauto. *)
-(*     + inv LOCAL0. ss. clarify. *)
-(*       exists mem_src, mem_src. splits; eauto. *)
-(*       econs; eauto. econs; eauto. *)
-(*     + inv LOCAL0. ss. clarify. *)
-(*       exists mem_src, mem_src. splits; eauto. *)
-(*       econs; eauto. econs; eauto. *)
-(* Qed. *)
+Admitted.
